strengthen tarjan low parent pending invariants

SeparationLogic/algorithms/Tarjan_directed/Tarjan_scc_is_low.v
@@ -1,11 +1,13 @@
 Require Import Coq.Classes.EquivDec.
 Require Import Coq.Lists.List.
 Require Import Coq.Logic.Classical_Prop.
+Require Import Coq.Arith.PeanoNat.
 Require Import Lia.
 Require Import SetsClass.SetsClass.
 From MonadLib.StateRelMonad Require Import StateRelBasic StateRelHoare FixpointLib.
 From GraphLib Require Import graph_basic Syntax.
 From GraphLib.examples Require Import tarjan.
+From MaxMinLib Require Import MaxMin Interface.
 From Algorithms.Tarjan_directed Require Import
   SCC_basic Tarjan_scc Tarjan_scc_basics Tarjan_scc_is_dfn
   Tarjan_scc_low_defs Tarjan_scc_low_pure Tarjan_scc_low_primitives.
@@ -1392,18 +1394,32 @@ Section IS_LOW.
              unfold wf_scc_state in Hwf.
              eapply Hpreloop; [| exact Hrun].
              split; [exact (Hframes cur s_cur Hin_tail) | split; [exact (proj1 Hwf) | exact Hnvis]].
-        * eapply Hoare_conseq
-            with (P2 := fun s => low_pre g root x s /\ stack_dfn_order s /\ dfn_injective s)
-                 (Q2 := fun _ s => low_iteration_entry g root x s).
-          intros s_pre Hpre.
-          subst s_pre.
-          destruct Hsnap as [[Hframes [Hwf [Hord Hinj]]] [Hlow Hbelow_timer]].
-          split; [exact Hlow | split; [exact Hord | exact Hinj]].
-          intros _ s Hentry.
-          unfold low_iteration_entry, low_iteration_inv in Hentry.
-          destruct Hentry as [[Hwf [_ [_ _]]] [Hord Hinj]].
-          split; [exact Hwf | split; [exact Hord | exact Hinj]].
-          apply (preloop_establishes_low_iteration_entry g root x).
+        * apply Hoare_conj with
+            (Q1 := fun _ s => wf_scc_state g root s)
+            (Q2 := fun _ s => stack_dfn_order s /\ dfn_injective s).
+          -- eapply Hoare_conseq_pre.
+             2: apply (preloop_preserves_wf_scc_state g root x).
+             intros s_pre Hpre.
+             subst s_pre.
+             destruct Hsnap as [[Hframes [Hwf [Hord Hinj]]] [Hlow Hbelow_timer]].
+             exact Hlow.
+          -- apply Hoare_conj.
+             ++ eapply Hoare_conseq_pre.
+                2: apply (preloop_preserves_stack_dfn_order x).
+                intros s_pre Hpre.
+                subst s_pre.
+                destruct Hsnap as [[Hframes [Hwf [Hord Hinj]]] [[_ Hnvis] Hbelow_timer]].
+                unfold wf_scc_state in Hwf.
+                destruct Hwf as [Hsiv [Hinv _]].
+                split; [exact Hord | split; [exact Hinv | split; [exact Hsiv | exact Hnvis]]].
+             ++ eapply Hoare_conseq_pre.
+                2: apply (preloop_preserves_dfn_injective x).
+                intros s_pre Hpre.
+                subst s_pre.
+                destruct Hsnap as [[Hframes [Hwf [Hord Hinj]]] [[_ Hnvis] Hbelow_timer]].
+                unfold wf_scc_state in Hwf.
+                destruct Hwf as [_ [Hinv _]].
+                split; [exact Hinj | split; [exact Hinv | exact Hnvis]].
       + unfold Hoare. intros s_pre r s_post Hpre Hrun.
         subst s_pre.
         unfold active_stack_frames_below.
@@ -1559,6 +1575,415 @@ Section IS_LOW.
           -- destruct H1 as [Heq _]. subst s. exact (proj2 H).
   Qed.
 
+  Definition no_new_parent_except
+             (parent root_child: V) (s0 s: @SCCSt V): Prop :=
+    forall v,
+      fa s v = parent ->
+      v <> parent ->
+      v <> root_child ->
+      v ∈ visited s0.
+
+  Lemma preloop_preserves_no_new_parent_except
+        (x parent root_child: V) (s0: @SCCSt V):
+    Hoare (fun s: @SCCSt V => s = s0 /\ no_new_parent_except parent root_child s0 s)
+          (preloop x)
+          (fun _ s => no_new_parent_except parent root_child s0 s).
+  Proof.
+    unfold Hoare.
+    intros s1 r s2 [Heq Hno] Hrun w Hfa_w Hw_ne_parent Hw_ne_root.
+    subst s1.
+    pose proof (preloop_keep_fa_no_restriction x w (fa s0 w)) as Hkeep.
+    unfold Hoare in Hkeep.
+    assert (Hfa_pres: fa s2 w = fa s0 w).
+    { eapply Hkeep; [reflexivity | exact Hrun]. }
+    apply Hno; auto.
+    rewrite <- Hfa_pres. exact Hfa_w.
+  Qed.
+
+  Lemma set_fa_preserves_no_new_parent_except
+        (v x parent root_child: V) (s0: @SCCSt V):
+    x <> parent ->
+    Hoare (fun s: @SCCSt V => no_new_parent_except parent root_child s0 s)
+          (set_fa v x)
+          (fun _ s => no_new_parent_except parent root_child s0 s).
+  Proof.
+    intros Hx_ne_parent.
+    unfold set_fa. intro_state. hoare_auto_s.
+    subst s. simpl.
+    unfold no_new_parent_except in *.
+    intros w Hfa_w Hw_ne_parent Hw_ne_root.
+    unfold equiv_decb in Hfa_w.
+    destruct (equiv_dec w v) as [Hw_eq_v | Hw_neq_v].
+    - destruct Hw_eq_v. simpl in Hfa_w.
+      unfold equiv_decb in Hfa_w.
+      destruct (equiv_dec w w) as [_ | Hneq].
+      + exfalso. apply Hx_ne_parent. exact Hfa_w.
+      + exfalso. apply Hneq. reflexivity.
+    - simpl in Hfa_w.
+      unfold equiv_decb in Hfa_w.
+      destruct (equiv_dec w v) as [Hw_eq_v' | _].
+      + exfalso. apply Hw_neq_v. exact Hw_eq_v'.
+      + apply H; auto.
+  Qed.
+
+  Lemma update_low_preserves_no_new_parent_except
+        (u parent root_child: V) (n: nat) (s0: @SCCSt V):
+    Hoare (fun s: @SCCSt V => no_new_parent_except parent root_child s0 s)
+          (update_low u n)
+          (fun _ s => no_new_parent_except parent root_child s0 s).
+  Proof.
+    unfold Hoare, no_new_parent_except.
+    intros s1 r s2 Hno Hrun w Hfa_w Hw_ne_parent Hw_ne_root.
+    pose proof (update_low_keep_fa u w n (fa s1 w)) as Hkeep.
+    unfold Hoare in Hkeep.
+    assert (Hfa_pres: fa s2 w = fa s1 w).
+    { eapply Hkeep; [reflexivity | exact Hrun]. }
+    apply Hno; auto.
+    rewrite <- Hfa_pres. exact Hfa_w.
+  Qed.
+
+  Lemma get_low_update_low_preserves_no_new_parent_except
+        (u v parent root_child: V) (s0: @SCCSt V):
+    Hoare (fun s: @SCCSt V => no_new_parent_except parent root_child s0 s)
+          (lv <- get' (fun s => low s v);; update_low u lv)
+          (fun _ s => no_new_parent_except parent root_child s0 s).
+  Proof.
+    apply Hoare_normalize. intros snap Hsnap.
+    eapply Hoare_bind. { eapply Hoare_get'. } simpl. intros lv.
+    eapply Hoare_conseq_pre.
+    2: { apply update_low_preserves_no_new_parent_except. }
+    intros st [Heq _]. subst st. exact Hsnap.
+  Qed.
+
+  Lemma get_dfn_update_low_preserves_no_new_parent_except
+        (u v parent root_child: V) (s0: @SCCSt V):
+    Hoare (fun s: @SCCSt V => no_new_parent_except parent root_child s0 s)
+          (dv <- get' (fun s => dfn s v);; update_low u dv)
+          (fun _ s => no_new_parent_except parent root_child s0 s).
+  Proof.
+    apply Hoare_normalize. intros snap Hsnap.
+    eapply Hoare_bind. { eapply Hoare_get'. } simpl. intros dv.
+    eapply Hoare_conseq_pre.
+    2: { apply update_low_preserves_no_new_parent_except. }
+    intros st [Heq _]. subst st. exact Hsnap.
+  Qed.
+
+  Lemma pop_scc_preserves_no_new_parent_except
+        (u parent root_child: V) (s0: @SCCSt V):
+    Hoare (fun s: @SCCSt V => no_new_parent_except parent root_child s0 s)
+          (pop_scc u)
+          (fun _ s => no_new_parent_except parent root_child s0 s).
+  Proof.
+    unfold Hoare, no_new_parent_except.
+    intros s1 r s2 Hno Hrun w Hfa_w Hw_ne_parent Hw_ne_root.
+    pose proof (pop_scc_keep_fa u w (fa s1 w)) as Hkeep.
+    unfold Hoare in Hkeep.
+    assert (Hfa_pres: fa s2 w = fa s1 w).
+    { eapply Hkeep; [reflexivity | exact Hrun]. }
+    apply Hno; auto.
+    rewrite <- Hfa_pres. exact Hfa_w.
+  Qed.
+
+  Lemma process_edge_preserves_no_new_parent_except
+        (u v parent root_child: V) (s0: @SCCSt V)
+        (W: V -> program (@SCCSt V) unit):
+    u <> parent ->
+    (forall x,
+       Hoare (fun s: @SCCSt V => no_new_parent_except parent root_child s0 s)
+             (W x)
+             (fun _ s => no_new_parent_except parent root_child s0 s)) ->
+    Hoare (fun s: @SCCSt V => no_new_parent_except parent root_child s0 s)
+          (process_edge u W v)
+          (fun _ s => no_new_parent_except parent root_child s0 s).
+  Proof.
+    intros Hu_ne_parent HW.
+    unfold process_edge, if_else, If.
+    intro_state.
+    apply Hoare_choice.
+    - apply Hoare_assume_bind. simpl.
+      apply Hoare_conseq_pre with
+        (P2 := fun s => no_new_parent_except parent root_child s0 s).
+      { intros st [_ Heq_st]. subst st. exact H. }
+      eapply Hoare_bind.
+      { apply set_fa_preserves_no_new_parent_except. exact Hu_ne_parent. }
+      simpl. intros _.
+      eapply Hoare_bind.
+      { apply HW. }
+      simpl. intros _.
+      exact (get_low_update_low_preserves_no_new_parent_except
+               u v parent root_child s0).
+    - apply Hoare_assume_bind. simpl.
+      apply Hoare_conseq_pre with
+        (P2 := fun s => no_new_parent_except parent root_child s0 s).
+      { intros st [_ Heq_st]. subst st. exact H. }
+      intro_state. hoare_auto_s.
+      + eapply Hoare_conseq_pre.
+        2: { exact (update_low_preserves_no_new_parent_except
+                      u parent root_child (dfn s2 v) s0). }
+        intros st Heq_st. subst st. exact H1.
+      + destruct H2 as [Heq _]. subst s. exact H1.
+  Qed.
+
+  Lemma forset_preserves_no_new_parent_except
+        (u parent root_child: V) (s0: @SCCSt V)
+        (W: V -> program (@SCCSt V) unit):
+    u <> parent ->
+    (forall x,
+       Hoare (fun s: @SCCSt V => no_new_parent_except parent root_child s0 s)
+             (W x)
+             (fun _ s => no_new_parent_except parent root_child s0 s)) ->
+    Hoare (fun s: @SCCSt V => no_new_parent_except parent root_child s0 s)
+          (forset (fun v => dg_step g u v) (process_edge u W))
+          (fun _ s => no_new_parent_except parent root_child s0 s).
+  Proof.
+    intros Hu_ne_parent HW.
+    unfold forset. hoare_fix_nolv_auto (V -> Prop).
+    simpl. intros W0 IH0 todo.
+    unfold forset_f. hoare_auto_s. intro_state. hoare_auto_s.
+    - eapply Hoare_bind.
+      { apply Hoare_conseq_pre with
+          (P2 := fun s => no_new_parent_except parent root_child s0 s).
+        { intros st Hst. subst st. exact H. }
+        apply process_edge_preserves_no_new_parent_except.
+        - exact Hu_ne_parent.
+        - intros x. apply HW. }
+      simpl. intros _. apply IH0.
+  Qed.
+
+  Lemma process_edge_preserves_parent_no_new_parent_except
+        (W: V -> program (@SCCSt V) unit)
+        (u v parent root_child: V) (s0: @SCCSt V):
+    u <> parent ->
+    (forall y,
+       Hoare (fun s: @SCCSt V =>
+                parent ∈ visited s /\
+                no_new_parent_except parent root_child s0 s)
+             (W y)
+             (fun _ s =>
+                parent ∈ visited s /\
+                no_new_parent_except parent root_child s0 s)) ->
+    Hoare (fun s: @SCCSt V =>
+             parent ∈ visited s /\
+             no_new_parent_except parent root_child s0 s)
+          (process_edge u W v)
+          (fun _ s =>
+             parent ∈ visited s /\
+             no_new_parent_except parent root_child s0 s).
+  Proof.
+    intros Hu_ne_parent HW.
+    unfold process_edge, if_else, If.
+    intro_state.
+    apply Hoare_choice.
+    - apply Hoare_assume_bind. simpl.
+      apply Hoare_conseq_pre with
+        (P2 := fun s =>
+                 parent ∈ visited s /\
+                 no_new_parent_except parent root_child s0 s).
+      { intros st [_ Heq_st]. subst st. exact H. }
+      eapply Hoare_bind.
+      { apply Hoare_conj.
+        - eapply Hoare_conseq_pre.
+          2: { apply set_fa_keep_visited. }
+          intros st [Hparent_vis _]. exact Hparent_vis.
+        - eapply Hoare_conseq_pre.
+          2: { apply set_fa_preserves_no_new_parent_except. exact Hu_ne_parent. }
+          intros st [_ Hno]. exact Hno. }
+      simpl. intros _.
+      eapply Hoare_bind.
+      { apply HW. }
+      simpl. intros _.
+      apply Hoare_conj.
+      + eapply Hoare_conseq_pre.
+        2: { apply get_low_update_low_keep_visited. }
+        intros st [Hparent_vis _]. exact Hparent_vis.
+      + eapply Hoare_conseq_pre.
+        2: { exact (get_low_update_low_preserves_no_new_parent_except
+                      u v parent root_child s0). }
+        intros st [_ Hno]. exact Hno.
+    - apply Hoare_assume_bind. simpl.
+      apply Hoare_conseq_pre with
+        (P2 := fun s =>
+                 parent ∈ visited s /\
+                 no_new_parent_except parent root_child s0 s).
+      { intros st [_ Heq_st]. subst st. exact H. }
+      intro_state. hoare_auto_s.
+      + apply Hoare_conj.
+        * eapply Hoare_conseq_pre.
+          2: { apply update_low_keep_visited. }
+          intros st Heq_st. subst st. exact (proj1 H1).
+        * eapply Hoare_conseq_pre.
+          2: { exact (update_low_preserves_no_new_parent_except
+                        u parent root_child (dfn s2 v) s0). }
+          intros st Heq_st. subst st. exact (proj2 H1).
+      + destruct H2 as [Heq _]. subst s. exact H1.
+  Qed.
+
+  Lemma forset_preserves_parent_no_new_parent_except
+        (W: V -> program (@SCCSt V) unit)
+        (x parent root_child: V) (s0: @SCCSt V):
+    x <> parent ->
+    (forall y,
+       Hoare (fun s: @SCCSt V =>
+                parent ∈ visited s /\
+                no_new_parent_except parent root_child s0 s)
+             (W y)
+             (fun _ s =>
+                parent ∈ visited s /\
+                no_new_parent_except parent root_child s0 s)) ->
+    Hoare (fun s: @SCCSt V =>
+             parent ∈ visited s /\
+             no_new_parent_except parent root_child s0 s)
+          (forset (fun v => dg_step g x v) (process_edge x W))
+          (fun _ s =>
+             parent ∈ visited s /\
+             no_new_parent_except parent root_child s0 s).
+  Proof.
+    intros Hx_ne_parent HW.
+    unfold forset. hoare_fix_nolv_auto (V -> Prop).
+    simpl. intros W0 IH0 todo.
+    unfold forset_f. hoare_auto_s. intro_state. hoare_auto_s.
+    eapply Hoare_bind.
+    { apply Hoare_conseq_pre with
+        (P2 := fun s =>
+                 parent ∈ visited s /\
+                 no_new_parent_except parent root_child s0 s).
+      { intros st Hst. subst st. exact H. }
+      apply process_edge_preserves_parent_no_new_parent_except.
+      - exact Hx_ne_parent.
+      - intros y. apply HW. }
+    simpl. intros _. apply IH0.
+  Qed.
+
+  Lemma tarjan_scc_f_preserves_parent_no_new_parent_except
+        (W: V -> program (@SCCSt V) unit)
+        (x parent root_child: V) (s0: @SCCSt V):
+    x <> parent ->
+    (forall y,
+       Hoare (fun s: @SCCSt V =>
+                parent ∈ visited s /\
+                no_new_parent_except parent root_child s0 s)
+             (W y)
+             (fun _ s =>
+                parent ∈ visited s /\
+                no_new_parent_except parent root_child s0 s)) ->
+    Hoare (fun s: @SCCSt V =>
+             s = s0 /\
+             parent ∈ visited s /\
+             no_new_parent_except parent root_child s0 s)
+          (tarjan_scc_f g W x)
+          (fun _ s =>
+             parent ∈ visited s /\
+             no_new_parent_except parent root_child s0 s).
+  Proof.
+    intros Hx_ne_parent HW.
+    unfold tarjan_scc_f.
+    eapply Hoare_bind.
+    - apply Hoare_conj.
+      + eapply Hoare_conseq_pre.
+        2: { apply preloop_keep_visited. }
+        intros st [_ [Hparent_vis _]]. exact Hparent_vis.
+      + eapply Hoare_conseq_pre.
+        2: { apply preloop_preserves_no_new_parent_except. }
+        intros st [Heq [_ Hno]]. split; [exact Heq | exact Hno].
+    - simpl. intros _.
+      eapply Hoare_bind.
+      + eapply Hoare_conseq_pre.
+        2: {
+          apply forset_preserves_parent_no_new_parent_except.
+          - exact Hx_ne_parent.
+          - intros y. apply HW.
+        }
+        intros st Hpair. exact Hpair.
+      + simpl. intros _.
+        unfold If. intro_state. hoare_auto_s.
+        * apply Hoare_conj.
+          -- eapply Hoare_conseq_pre.
+             2: { apply pop_scc_keep_visited. }
+             intros st Heq. subst st. exact (proj1 H).
+          -- eapply Hoare_conseq_pre.
+             2: { apply pop_scc_preserves_no_new_parent_except. }
+             intros st Heq. subst st. exact (proj2 H).
+        * destruct H1 as [Heq _]. subst s. exact H.
+  Qed.
+
+  Lemma no_new_parent_except_implies_fa_child_of_u
+        (u a: V) (snap s: @SCCSt V):
+    fa_child_of_u g u snap ->
+    dg_step g u a ->
+    (forall v, v ∈ visited snap -> fa s v = fa snap v) ->
+    no_new_parent_except u a snap s ->
+    fa_child_of_u g u s.
+  Proof.
+    intros Hchild Hdg Hstable Hno v [Hfa_v Hfa_neq_v].
+    destruct (equiv_dec v a) as [Hv_eq_a | Hv_neq_a].
+    - rewrite Hv_eq_a. exact Hdg.
+    - assert (Hv_neq_u: v <> u).
+      { intro Hv_eq_u. apply Hfa_neq_v. rewrite Hfa_v. symmetry. exact Hv_eq_u. }
+      assert (Hvis_snap: v ∈ visited snap).
+      { apply (Hno v Hfa_v Hv_neq_u Hv_neq_a). }
+      apply (Hchild v).
+      split.
+      + rewrite <- (Hstable v Hvis_snap). exact Hfa_v.
+      + intro Hloop_snap.
+        apply Hfa_neq_v.
+        rewrite (Hstable v Hvis_snap).
+        exact Hloop_snap.
+  Qed.
+
+  Lemma no_new_parent_except_implies_fa_not_done
+        (u a: V) (done: V -> Prop) (snap s: @SCCSt V):
+    fa_not_done_implies_eq_u u (done ∪ [a]) snap ->
+    (forall v, v ∈ visited snap -> fa s v = fa snap v) ->
+    no_new_parent_except u a snap s ->
+    fa_not_done_implies_eq_u u (done ∪ [a]) s.
+  Proof.
+    intros Hfa_not Hstable Hno v Hnot_done Hfa_v.
+    destruct (equiv_dec v u) as [Hv_eq_u | Hv_neq_u].
+    - exact Hv_eq_u.
+    - assert (Hv_neq_a: v <> a).
+      { intro Hv_eq_a. apply Hnot_done. sets_unfold. right. symmetry. exact Hv_eq_a. }
+      assert (Hvis_snap: v ∈ visited snap).
+      { apply (Hno v Hfa_v Hv_neq_u Hv_neq_a). }
+      apply Hfa_not.
+      + exact Hnot_done.
+      + rewrite <- (Hstable v Hvis_snap). exact Hfa_v.
+  Qed.
+
+  Lemma tarjan_scc_preserves_old_vertex_data
+        (a v: V) (snap: @SCCSt V):
+    a <> v ->
+    v ∈ visited snap ->
+    Hoare (fun s: @SCCSt V => s = snap)
+          (tarjan_scc g a)
+          (fun _ s =>
+             v ∈ visited s /\
+             dfn s v = dfn snap v /\
+             low s v = low snap v /\
+             fa s v = fa snap v).
+  Proof.
+    intros Ha_ne_v Hvvis.
+    unfold Hoare.
+    intros s1 r s2 Heq Hrun.
+    subst s1.
+    pose proof (tarjan_scc_keep_dfn g a v (dfn snap v)) as Hdfn_keep.
+    pose proof (tarjan_scc_keep_low g a v (low snap v)) as Hlow_keep.
+    pose proof (Tarjan_scc_basics.tarjan_scc_keep_fa g a v (fa snap v)) as Hfa_keep.
+    unfold Hoare in Hdfn_keep, Hlow_keep, Hfa_keep.
+    specialize (Hdfn_keep snap r s2).
+    specialize (Hlow_keep snap r s2).
+    specialize (Hfa_keep snap r s2).
+    assert (Hdfn_post: v ∈ visited s2 /\ dfn s2 v = dfn snap v).
+    { apply Hdfn_keep; [repeat split; auto | exact Hrun]. }
+    assert (Hlow_post: v ∈ visited s2 /\ low s2 v = low snap v).
+    { apply Hlow_keep; [repeat split; auto | exact Hrun]. }
+    assert (Hfa_post: v ∈ visited s2 /\ fa s2 v = fa snap v).
+    { apply Hfa_keep; [repeat split; auto | exact Hrun]. }
+    destruct Hdfn_post as [Hvis Hdfn].
+    destruct Hlow_post as [_ Hlow].
+    destruct Hfa_post as [_ Hfa].
+    split; [exact Hvis | split; [exact Hdfn | split; [exact Hlow | exact Hfa]]].
+  Qed.
+
   (* ================================================================ *)
   (* Forset phase contracts                                          *)
   (* ================================================================ *)
@@ -1585,9 +2010,11 @@ Section IS_LOW.
   Definition low_tree_child_after_set_fa
              (u a: V) (done: V -> Prop) (s: @SCCSt V): Prop :=
     wf_scc_state_pre g root a s /\
+    settled_closed g s /\
     u ∈ visited s /\
     In u (stack s) /\
     done_visited done s /\
+    done_reachable_closed g done s /\
     low_frontier g u done s /\
     low_src g u done s /\
     children_low_valid g root u done s /\
@@ -1600,9 +2027,11 @@ Section IS_LOW.
   Definition low_tree_child_parent_pending
              (u a: V) (done: V -> Prop) (s: @SCCSt V): Prop :=
     wf_scc_state g root s /\
+    settled_closed g s /\
     u ∈ visited s /\
     In u (stack s) /\
     done_visited done s /\
+    done_reachable_closed g done s /\
     low_frontier g u done s /\
     low_src g u done s /\
     children_low_valid g root u done s /\
@@ -1659,48 +2088,55 @@ Section IS_LOW.
       dfn_injective s.
   Proof.
     intros s Hiter Hord Hinj Hdg Hndone Hvis Hnot_stack.
-    destruct Hiter as (Hwf & Huvis & Hustack & Hdonevis & Hfront & Hsrc &
-                       Hchild & Hfa_child & Hfa_not).
+    destruct Hiter as (Hwf & Hsettled & Huvis & Hustack & Hdonevis &
+                       Hclosed & Hfront & Hsrc & Hchild & Hfa_child &
+                       Hfa_not).
     split; [| split; [exact Hord | exact Hinj]].
     unfold low_iteration_inv.
-    split; [exact Hwf | split; [exact Huvis | split; [exact Hustack |]]].
+    split; [exact Hwf | split; [exact Hsettled | split; [exact Huvis | split; [exact Hustack |]]]].
     split.
     - unfold done_visited in Hdonevis |- *.
       intros w Hw. sets_unfold in Hw. destruct Hw as [Hdone_w | Hw_eq].
       + apply Hdonevis. exact Hdone_w.
       + subst w. exact Hvis.
     - split.
-      + unfold low_frontier in Hfront |- *.
+      + unfold done_reachable_closed in Hclosed |- *.
+        intros v w Hv_done Hreach.
+        sets_unfold in Hv_done. destruct Hv_done as [Hv_done | Hv_eq].
+        * eapply Hclosed; eauto.
+        * subst v. eapply Hsettled; eauto.
+      + split.
+        * unfold low_frontier in Hfront |- *.
         destruct Hfront as [Hle Hfront]. split; [exact Hle |].
         intros v Hv_done Hv_dg.
         sets_unfold in Hv_done. destruct Hv_done as [Hv_done | Hv_eq].
-        * apply Hfront; auto.
-        * subst v. split.
-          -- intro Hfa_a.
-             specialize (Hfa_not a Hndone Hfa_a). subst a.
-             contradiction.
-          -- intro Ha_stack. contradiction.
-      + split.
-        * unfold low_src in Hsrc |- *.
+        -- apply Hfront; auto.
+        -- subst v. split.
+           ++ intro Hfa_a.
+              specialize (Hfa_not a Hndone Hfa_a). subst a.
+              contradiction.
+           ++ intro Ha_stack. contradiction.
+        * split.
+          -- unfold low_src in Hsrc |- *.
           destruct Hsrc as [Hsrc | [(v & Hdone_v & Hdg_v & Hfa_v & Hfa_neq_v & Hlow_v) |
                                    (w & Hdone_w & Hdg_w & Hstack_w & Hfa_neq_w & Hlow_w)]].
-          -- left. exact Hsrc.
-          -- right. left. exists v. repeat split; auto. sets_unfold. left. exact Hdone_v.
-          -- right. right. exists w. repeat split; auto. sets_unfold. left. exact Hdone_w.
-        * split.
-          -- unfold children_low_valid in Hchild |- *.
+          ++ left. exact Hsrc.
+          ++ right. left. exists v. repeat split; auto. sets_unfold. left. exact Hdone_v.
+          ++ right. right. exists w. repeat split; auto. sets_unfold. left. exact Hdone_w.
+          -- split.
+             ++ unfold children_low_valid in Hchild |- *.
              intros v Hv_done Hv_dg Hfa_v Hfa_neq_v.
              sets_unfold in Hv_done. destruct Hv_done as [Hv_done | Hv_eq].
-             ++ apply Hchild; auto.
-             ++ subst v.
+             ** apply Hchild; auto.
+             ** subst v.
                 specialize (Hfa_not a Hndone Hfa_v). subst a.
                 contradiction.
-          -- split.
-             ++ exact Hfa_child.
-             ++ unfold fa_not_done_implies_eq_u in Hfa_not |- *.
-                intros v Hnot_done Hfa_v.
-                apply Hfa_not; [| exact Hfa_v].
-                intro Hdone_v. apply Hnot_done. sets_unfold. left. exact Hdone_v.
+             ++ split.
+                ** exact Hfa_child.
+                ** unfold fa_not_done_implies_eq_u in Hfa_not |- *.
+                   intros v Hnot_done Hfa_v.
+                   apply Hfa_not; [| exact Hfa_v].
+                   intro Hdone_v. apply Hnot_done. sets_unfold. left. exact Hdone_v.
   Qed.
 
   Lemma low_iteration_extend_done_skip_nonstack
@@ -1770,22 +2206,29 @@ Section IS_LOW.
       subst s.
       unfold RecordSet.set. simpl.
       destruct Hsnap as [Hiter [Hord [Hinj [Hdg [Hndone [Hvis Hstack_a]]]]]].
-      destruct Hiter as (Hwf & Huvis & Hustack & Hdonevis & Hfront & Hsrc &
-                         Hchild & Hfa_child & Hfa_not).
+      destruct Hiter as (Hwf & Hsettled & Huvis & Hustack & Hdonevis &
+                         Hclosed & Hfront & Hsrc & Hchild & Hfa_child &
+                         Hfa_not).
       split; [| split].
       + unfold low_iteration_inv.
         split.
         * unfold wf_scc_state in Hwf |- *.
           destruct Hwf as [Hsiv [Hinv [Hvalid Hfa_vis]]].
           split; [exact Hsiv | split; [exact Hinv | split; [exact Hvalid | exact Hfa_vis]]].
-        * split; [exact Huvis | split; [exact Hustack |]].
+        * split; [exact Hsettled | split; [exact Huvis | split; [exact Hustack |]]].
           split.
           -- unfold done_visited in Hdonevis |- *.
              intros w Hw. sets_unfold in Hw. destruct Hw as [Hdone_w | Hw_eq].
              ++ apply Hdonevis. exact Hdone_w.
              ++ subst w. exact Hvis.
           -- split.
-             ++ unfold low_frontier in Hfront |- *.
+             ++ unfold done_reachable_closed in Hclosed |- *.
+                intros v w Hv_done Hnot_stack_v Hreach.
+                sets_unfold in Hv_done. destruct Hv_done as [Hv_done | Hv_eq].
+                ** eapply Hclosed; eauto.
+                ** subst v. contradiction.
+             ++ split.
+                ** unfold low_frontier in Hfront |- *.
                 destruct Hfront as [Hle Hfront].
                 split.
                 { simpl. unfold equiv_decb.
@@ -1794,7 +2237,7 @@ Section IS_LOW.
                     | exfalso; apply Hc; reflexivity]. }
                 intros v Hv_done Hv_dg.
                 sets_unfold in Hv_done. destruct Hv_done as [Hv_done | Hv_eq].
-                ** specialize (Hfront v Hv_done Hv_dg) as [Hfa_part Hstack_part].
+                { specialize (Hfront v Hv_done Hv_dg) as [Hfa_part Hstack_part].
                    split; intros Hcase.
                    --- simpl. unfold equiv_decb.
                        destruct (equiv_dec u u) as [_ | Hc];
@@ -1807,8 +2250,8 @@ Section IS_LOW.
                        destruct (equiv_dec u u) as [_ | Hc];
                          [assert (dfn snap a <= dfn snap v) by
                             (pose proof (Hstack_part Hcase); lia); exact H
-                         | exfalso; apply Hc; reflexivity].
-                ** subst v.
+                         | exfalso; apply Hc; reflexivity]. }
+                { subst v.
                    split;
                      [ intros Hfa_a;
                        simpl; unfold equiv_decb;
@@ -1820,9 +2263,9 @@ Section IS_LOW.
                      | intros _;
                        simpl; unfold equiv_decb;
                        destruct (equiv_dec u u) as [_ | Hc];
-                       [ lia | exfalso; apply Hc; reflexivity ] ].
-             ++ split.
-                ** unfold low_src in Hsrc |- *.
+                       [ lia | exfalso; apply Hc; reflexivity ] ]. }
+                ** split.
+                   --- unfold low_src in Hsrc |- *.
                    unfold equiv_decb.
                    destruct (equiv_dec u u) as [_ | Hc]; [| exfalso; apply Hc; reflexivity].
 	                   destruct (equiv_dec a u) as [Ha_eq_u | Ha_neq_u].
@@ -1840,8 +2283,8 @@ Section IS_LOW.
 		                         [destruct (equiv_dec a u) as [Ha_eq_u' | Ha_neq_u'];
 		                          [contradiction | reflexivity]
 		                         | exfalso; apply Hc; reflexivity]. }
-                ** split.
-	                   --- unfold children_low_valid in Hchild |- *.
+                   --- split.
+	                   +++ unfold children_low_valid in Hchild |- *.
 	                       intros v Hv_done Hv_dg Hfa_v Hfa_neq_v.
 	                       sets_unfold in Hv_done. destruct Hv_done as [Hv_done | Hv_eq].
 	                       { apply (set_low_preserves_scc_low_valid_v_when_not_child g root v u (dfn snap a) snap).
@@ -1865,7 +2308,7 @@ Section IS_LOW.
 	                         - simpl in Hfa_v.
 	                           rewrite <- Hv_eq in Hfa_v.
 	                           specialize (Hfa_not a Hndone Hfa_v). contradiction. }
-	                   --- split.
+	                   +++ split.
 	                       { exact Hfa_child. }
 	                       { unfold fa_not_done_implies_eq_u in Hfa_not |- *.
 	                         intros v Hnot_done Hfa_v.
@@ -1875,52 +2318,59 @@ Section IS_LOW.
       + exact Hinj.
     - destruct H1 as [Heq_state Hnot_lt]. subst s.
       destruct Hsnap as [Hiter [Hord [Hinj [Hdg [Hndone [Hvis Hstack_a]]]]]].
-      destruct Hiter as (Hwf & Huvis & Hustack & Hdonevis & Hfront & Hsrc &
-                         Hchild & Hfa_child & Hfa_not).
+      destruct Hiter as (Hwf & Hsettled & Huvis & Hustack & Hdonevis &
+                         Hclosed & Hfront & Hsrc & Hchild & Hfa_child &
+                         Hfa_not).
       destruct H as [Heq_snap Hdv]. subst s0. subst dv.
       split; [| split; [exact Hord | exact Hinj]].
       unfold low_iteration_inv.
-      split; [exact Hwf | split; [exact Huvis | split; [exact Hustack |]]].
+      split; [exact Hwf | split; [exact Hsettled | split; [exact Huvis | split; [exact Hustack |]]]].
       split.
       + unfold done_visited in Hdonevis |- *.
         intros w Hw. sets_unfold in Hw. destruct Hw as [Hdone_w | Hw_eq].
         * apply Hdonevis. exact Hdone_w.
         * subst w. exact Hvis.
       + split.
-        * unfold low_frontier in Hfront |- *.
+        * unfold done_reachable_closed in Hclosed |- *.
+          intros v w Hv_done Hnot_stack_v Hreach.
+          sets_unfold in Hv_done. destruct Hv_done as [Hv_done | Hv_eq].
+          { eapply Hclosed; eauto. }
+          { subst v. contradiction. }
+        * split.
+          { unfold low_frontier in Hfront |- *.
           destruct Hfront as [Hle Hfront]. split; [exact Hle |].
           intros v Hv_done Hv_dg.
           sets_unfold in Hv_done. destruct Hv_done as [Hv_done | Hv_eq].
-          -- apply Hfront; auto.
-          -- subst v. split.
-	             ++ intro Hfa_a.
-	                destruct (equiv_dec a u) as [Ha_eq_u | Ha_neq_u].
-	                ** rewrite Ha_eq_u. lia.
-	                ** specialize (Hfa_not a Hndone Hfa_a). contradiction.
-	             ++ intro Hstack_a'. lia.
-        * split.
-          -- unfold low_src in Hsrc |- *.
+          { apply Hfront; auto. }
+          { subst v. split.
+            - intro Hfa_a.
+              destruct (equiv_dec a u) as [Ha_eq_u | Ha_neq_u].
+              + rewrite Ha_eq_u. lia.
+              + specialize (Hfa_not a Hndone Hfa_a). contradiction.
+            - intro Hstack_a'. lia. } }
+          { split.
+            - unfold low_src in Hsrc |- *.
              destruct Hsrc as [Hsrc | [(v & Hdone_v & Hdg_v & Hfa_v & Hfa_neq_v & Hlow_v) |
                                       (w & Hdone_w & Hdg_w & Hstack_w & Hfa_neq_w & Hlow_w)]].
-             ++ left. exact Hsrc.
-             ++ right. left. exists v. repeat split; auto. sets_unfold. left. exact Hdone_v.
-             ++ right. right. exists w. repeat split; auto. sets_unfold. left. exact Hdone_w.
-          -- split.
-             ++ unfold children_low_valid in Hchild |- *.
+             + left. exact Hsrc.
+             + right. left. exists v. repeat split; auto. sets_unfold. left. exact Hdone_v.
+             + right. right. exists w. repeat split; auto. sets_unfold. left. exact Hdone_w.
+            - split.
+              + unfold children_low_valid in Hchild |- *.
                 intros v Hv_done Hv_dg Hfa_v Hfa_neq_v.
                 sets_unfold in Hv_done. destruct Hv_done as [Hv_done | Hv_eq].
-                ** apply Hchild; auto.
-	                ** subst v.
-	                   destruct (equiv_dec a u) as [Ha_eq_u | Ha_neq_u].
-	                   --- exfalso. apply Hfa_neq_v.
-	                       rewrite Hfa_v. symmetry. exact Ha_eq_u.
-	                   --- specialize (Hfa_not a Hndone Hfa_v). contradiction.
-             ++ split.
-                ** exact Hfa_child.
-                ** unfold fa_not_done_implies_eq_u in Hfa_not |- *.
-                   intros v Hnot_done Hfa_v.
-                   apply Hfa_not; [| exact Hfa_v].
-                   intro Hdone_v. apply Hnot_done. sets_unfold. left. exact Hdone_v.
+                { apply Hchild; auto. }
+                { subst v.
+                  destruct (equiv_dec a u) as [Ha_eq_u | Ha_neq_u].
+                  - exfalso. apply Hfa_neq_v.
+                    rewrite Hfa_v. symmetry. exact Ha_eq_u.
+                  - specialize (Hfa_not a Hndone Hfa_v). contradiction. }
+              + split.
+                * exact Hfa_child.
+                * unfold fa_not_done_implies_eq_u in Hfa_not |- *.
+                  intros v Hnot_done Hfa_v.
+                  apply Hfa_not; [| exact Hfa_v].
+                  intro Hdone_v. apply Hnot_done. sets_unfold. left. exact Hdone_v. }
   Qed.
 
   Lemma get_low_update_low_tree_child_extends_low_iteration
@@ -1937,11 +2387,12 @@ Section IS_LOW.
     unfold update_low. unfold_op. intro_state. hoare_auto_s.
     - destruct H as [Heq_snap Hlv]. subst s0. subst lv.
       subst s. unfold RecordSet.set. simpl.
-      destruct Hsnap as [Hpending Hvalid_a].
-      destruct Hpending as
-        (Hwf & Huvis & Hustack & Hdonevis & Hfront & Hsrc & Hchild &
-         Hfa_child & Hfa_not & Hord & Hinj & Hdg & Hndone & Hvis &
-         Hfa_a & Hfa_neq_a).
+	      destruct Hsnap as [Hpending Hvalid_a].
+	      destruct Hpending as
+	        (Hwf & Hsettled & Huvis & Hustack & Hdonevis & Hclosed &
+           Hfront & Hsrc & Hchild &
+	         Hfa_child & Hfa_not & Hord & Hinj & Hdg & Hndone & Hvis &
+	         Hfa_a & Hfa_neq_a).
       assert (Ha_neq_u: a <> u).
       { intro Ha_eq. subst a. apply Hfa_neq_a. exact Hfa_a. }
       assert (Hlow_a_dfn_a: low snap a <= dfn snap a).
@@ -1955,25 +2406,31 @@ Section IS_LOW.
       + unfold wf_scc_state in Hwf |- *.
         destruct Hwf as [Hsiv [Hinv [Hvalid Hfa_vis]]].
         split; [exact Hsiv | split; [exact Hinv | split; [exact Hvalid | exact Hfa_vis]]].
-      + split; [exact Huvis | split; [exact Hustack |]].
-        split.
-        * unfold done_visited in Hdonevis |- *.
-          intros w Hw. sets_unfold in Hw. destruct Hw as [Hdone_w | Hw_eq].
-          -- apply Hdonevis. exact Hdone_w.
-          -- subst w. exact Hvis.
-        * split.
-          -- unfold low_frontier in Hfront |- *.
-             destruct Hfront as [Hle Hfront].
-             split.
-             ++ simpl. unfold equiv_decb.
-                destruct (equiv_dec u u) as [_ | Hc];
-                  [lia | exfalso; apply Hc; reflexivity].
-             ++ intros v Hv_done Hv_dg.
-                sets_unfold in Hv_done. destruct Hv_done as [Hv_done | Hv_eq].
-                ** specialize (Hfront v Hv_done Hv_dg) as [Hfa_part Hstack_part].
-                   split.
-                   { intros Hcase.
-                       simpl. unfold equiv_decb.
+	      + split; [exact Hsettled | split; [exact Huvis | split; [exact Hustack |]]].
+	        split.
+	        * unfold done_visited in Hdonevis |- *.
+	          intros w Hw. sets_unfold in Hw. destruct Hw as [Hdone_w | Hw_eq].
+	          -- apply Hdonevis. exact Hdone_w.
+	          -- subst w. exact Hvis.
+	        * split.
+	          -- unfold done_reachable_closed in Hclosed |- *.
+	             intros v w Hv_done Hnot_stack_v Hreach.
+	             sets_unfold in Hv_done. destruct Hv_done as [Hv_done | Hv_eq].
+	             ++ eapply Hclosed; eauto.
+	             ++ subst v. eapply Hsettled; eauto.
+	          -- split.
+	             ++ unfold low_frontier in Hfront |- *.
+	             destruct Hfront as [Hle Hfront].
+	             split.
+	             ** simpl. unfold equiv_decb.
+	                destruct (equiv_dec u u) as [_ | Hc];
+	                  [lia | exfalso; apply Hc; reflexivity].
+	             ** intros v Hv_done Hv_dg.
+	                sets_unfold in Hv_done. destruct Hv_done as [Hv_done | Hv_eq].
+	                --- specialize (Hfront v Hv_done Hv_dg) as [Hfa_part Hstack_part].
+	                   split.
+	                   { intros Hcase.
+	                       simpl. unfold equiv_decb.
                        destruct (equiv_dec u u) as [_ | Hc].
                        - destruct (equiv_dec v u) as [Hv_eq_u | Hv_neq_u].
                          + lia.
@@ -1982,107 +2439,112 @@ Section IS_LOW.
                    { intros Hcase.
                        simpl. unfold equiv_decb.
                        destruct (equiv_dec u u) as [_ | Hc].
-                       - pose proof (Hstack_part Hcase). lia.
-                       - exfalso. apply Hc. reflexivity. }
-                ** subst v. split; intros _.
-                   --- simpl. unfold equiv_decb.
-                       destruct (equiv_dec u u) as [_ | Hc];
-                         [destruct (equiv_dec a u) as [Ha_eq_u | _];
-                          [exfalso; apply Ha_neq_u; exact Ha_eq_u | lia]
-                         | exfalso; apply Hc; reflexivity].
-                   --- simpl. unfold equiv_decb.
-                       destruct (equiv_dec u u) as [_ | Hc];
-                         [lia | exfalso; apply Hc; reflexivity].
-          -- split.
-             ++ unfold low_src.
-                right. left. exists a.
-                split; [sets_unfold; right; reflexivity |].
-                split; [exact Hdg |].
-                split.
-                { simpl. unfold equiv_decb.
-                   destruct (equiv_dec a u) as [Ha_eq_u | _].
-                   - exfalso. apply Ha_neq_u. exact Ha_eq_u.
-                   - exact Hfa_a. }
-                ** split.
-                   { simpl. unfold equiv_decb.
-                       destruct (equiv_dec a u) as [Ha_eq_u | _].
-                       - exfalso. apply Ha_neq_u. exact Ha_eq_u.
-                       - exact Hfa_neq_a. }
-                   { simpl. unfold equiv_decb.
-                       destruct (equiv_dec u u) as [_ | Hc];
-                         [destruct (equiv_dec a u) as [Ha_eq_u | _];
-                          [exfalso; apply Ha_neq_u; exact Ha_eq_u | reflexivity]
-                         | exfalso; apply Hc; reflexivity]. }
-             ++ split.
-                ** unfold children_low_valid in Hchild |- *.
-                   intros v Hv_done Hv_dg Hfa_v Hfa_neq_v.
-                   sets_unfold in Hv_done. destruct Hv_done as [Hv_done | Hv_eq].
-                   { apply (set_low_preserves_scc_low_valid_v_when_not_child g root v u (low snap a) snap).
-                     - intro Hv_eq_u. destruct Hv_eq_u. apply Hfa_neq_v. exact Hfa_v.
-                     - intro Htree_vu.
-                         unfold wf_scc_state in Hwf.
-                         destruct Hwf as [_ [_ [Hvalid _]]].
-                         assert (Hvu_lt: dfn snap v < dfn snap u).
-                         { apply Hvalid. exact Htree_vu. }
-                         assert (Huv_lt: dfn snap u < dfn snap v).
-                         { eapply fa_parent_dfn_lt; eauto. }
-                         lia.
-                     - apply Hchild; auto. }
-                   { subst v.
-                     apply (set_low_preserves_scc_low_valid_v_when_not_child g root a u (low snap a) snap).
-                     - exact Ha_neq_u.
-                     - intro Htree_au.
-                         unfold wf_scc_state in Hwf.
-                         destruct Hwf as [_ [_ [Hvalid _]]].
-                         assert (Hau_lt: dfn snap a < dfn snap u).
-                         { apply Hvalid. exact Htree_au. }
-                         lia.
-                     - exact Hvalid_a. }
-                ** split.
-                   --- exact Hfa_child.
-                   --- exact Hfa_not.
+	                       - pose proof (Hstack_part Hcase). lia.
+	                       - exfalso. apply Hc. reflexivity. }
+	                --- subst v. split; intros _.
+	                   +++ simpl. unfold equiv_decb.
+	                       destruct (equiv_dec u u) as [_ | Hc];
+	                         [destruct (equiv_dec a u) as [Ha_eq_u | _];
+	                          [exfalso; apply Ha_neq_u; exact Ha_eq_u | lia]
+	                         | exfalso; apply Hc; reflexivity].
+	                   +++ simpl. unfold equiv_decb.
+	                       destruct (equiv_dec u u) as [_ | Hc];
+	                         [lia | exfalso; apply Hc; reflexivity].
+	             ++ split.
+	                { unfold low_src.
+                    right. left. exists a.
+                    split; [sets_unfold; right; reflexivity |].
+                    split; [exact Hdg |].
+                    split.
+                    { simpl. unfold equiv_decb.
+                      destruct (equiv_dec a u) as [Ha_eq_u | _].
+                      - exfalso. apply Ha_neq_u. exact Ha_eq_u.
+                      - exact Hfa_a. }
+                    split.
+                    { simpl. unfold equiv_decb.
+                      destruct (equiv_dec a u) as [Ha_eq_u | _].
+                      - exfalso. apply Ha_neq_u. exact Ha_eq_u.
+                      - exact Hfa_neq_a. }
+                    { simpl. unfold equiv_decb.
+                      destruct (equiv_dec u u) as [_ | Hc];
+                        [destruct (equiv_dec a u) as [Ha_eq_u | _];
+                         [exfalso; apply Ha_neq_u; exact Ha_eq_u | reflexivity]
+                        | exfalso; apply Hc; reflexivity]. } }
+	                { split.
+	                  { unfold children_low_valid in Hchild |- *.
+	                    intros v Hv_done Hv_dg Hfa_v Hfa_neq_v.
+	                    sets_unfold in Hv_done. destruct Hv_done as [Hv_done | Hv_eq].
+	                    - apply (set_low_preserves_scc_low_valid_v_when_not_child g root v u (low snap a) snap).
+	                      + intro Hv_eq_u. destruct Hv_eq_u. apply Hfa_neq_v. exact Hfa_v.
+	                      + intro Htree_vu.
+	                        unfold wf_scc_state in Hwf.
+	                        destruct Hwf as [_ [_ [Hvalid _]]].
+	                        assert (Hvu_lt: dfn snap v < dfn snap u).
+	                        { apply Hvalid. exact Htree_vu. }
+	                        assert (Huv_lt: dfn snap u < dfn snap v).
+	                        { eapply fa_parent_dfn_lt; eauto. }
+	                        lia.
+	                      + apply Hchild; auto.
+	                    - subst v.
+	                      apply (set_low_preserves_scc_low_valid_v_when_not_child g root a u (low snap a) snap).
+	                      + exact Ha_neq_u.
+	                      + intro Htree_au.
+	                        unfold wf_scc_state in Hwf.
+	                        destruct Hwf as [_ [_ [Hvalid _]]].
+	                        assert (Hau_lt: dfn snap a < dfn snap u).
+	                        { apply Hvalid. exact Htree_au. }
+	                        lia.
+	                      + exact Hvalid_a. }
+	                  { split; [exact Hfa_child | exact Hfa_not]. } }
     - destruct H1 as [Heq_state Hnot_lt]. subst s.
-      destruct H as [Heq_snap Hlv]. subst s0. subst lv.
-      destruct Hsnap as [Hpending Hvalid_a].
-      destruct Hpending as
-        (Hwf & Huvis & Hustack & Hdonevis & Hfront & Hsrc & Hchild &
-         Hfa_child & Hfa_not & Hord & Hinj & Hdg & Hndone & Hvis &
-         Hfa_a & Hfa_neq_a).
+	      destruct H as [Heq_snap Hlv]. subst s0. subst lv.
+	      destruct Hsnap as [Hpending Hvalid_a].
+	      destruct Hpending as
+	        (Hwf & Hsettled & Huvis & Hustack & Hdonevis & Hclosed &
+           Hfront & Hsrc & Hchild &
+	         Hfa_child & Hfa_not & Hord & Hinj & Hdg & Hndone & Hvis &
+	         Hfa_a & Hfa_neq_a).
       assert (Ha_neq_u: a <> u).
       { intro Ha_eq. subst a. apply Hfa_neq_a. exact Hfa_a. }
       assert (Hlow_a_dfn_a: low snap a <= dfn snap a).
       { apply (scc_low_valid_v_bound_self g root). exact Hvalid_a. }
       split; [| split; [exact Hord | exact Hinj]].
       unfold low_iteration_inv.
-      split; [exact Hwf | split; [exact Huvis | split; [exact Hustack |]]].
-      split.
-      + unfold done_visited in Hdonevis |- *.
-        intros w Hw. sets_unfold in Hw. destruct Hw as [Hdone_w | Hw_eq].
-        * apply Hdonevis. exact Hdone_w.
-        * subst w. exact Hvis.
-      + split.
-        * unfold low_frontier in Hfront |- *.
-          destruct Hfront as [Hle Hfront]. split; [exact Hle |].
-          intros v Hv_done Hv_dg.
-          sets_unfold in Hv_done. destruct Hv_done as [Hv_done | Hv_eq].
-          { apply Hfront; auto. }
-          { subst v. split; intros; lia. }
-        * split.
-          -- unfold low_src in Hsrc |- *.
-             destruct Hsrc as [Hsrc | [(v & Hdone_v & Hdg_v & Hfa_v & Hfa_neq_v & Hlow_v) |
-                                      (w & Hdone_w & Hdg_w & Hstack_w & Hfa_neq_w & Hlow_w)]].
-             ++ left. exact Hsrc.
-             ++ right. left. exists v. repeat split; auto. sets_unfold. left. exact Hdone_v.
-             ++ right. right. exists w. repeat split; auto. sets_unfold. left. exact Hdone_w.
-          -- split.
-             ++ unfold children_low_valid in Hchild |- *.
-                intros v Hv_done Hv_dg Hfa_v Hfa_neq_v.
-                sets_unfold in Hv_done. destruct Hv_done as [Hv_done | Hv_eq].
-                ** apply Hchild; auto.
-                ** subst v. exact Hvalid_a.
-             ++ split.
-                ** exact Hfa_child.
-                ** exact Hfa_not.
+	      split; [exact Hwf | split; [exact Hsettled | split; [exact Huvis | split; [exact Hustack |]]]].
+	      split.
+	      + unfold done_visited in Hdonevis |- *.
+	        intros w Hw. sets_unfold in Hw. destruct Hw as [Hdone_w | Hw_eq].
+	        * apply Hdonevis. exact Hdone_w.
+	        * subst w. exact Hvis.
+	      + split.
+	        * unfold done_reachable_closed in Hclosed |- *.
+	          intros v w Hv_done Hnot_stack_v Hreach.
+	          sets_unfold in Hv_done. destruct Hv_done as [Hv_done | Hv_eq].
+	          -- eapply Hclosed; eauto.
+	          -- subst v. eapply Hsettled; eauto.
+	        * split.
+	          -- unfold low_frontier in Hfront |- *.
+	          destruct Hfront as [Hle Hfront]. split; [exact Hle |].
+	          intros v Hv_done Hv_dg.
+	          sets_unfold in Hv_done. destruct Hv_done as [Hv_done | Hv_eq].
+	          { apply Hfront; auto. }
+	          { subst v. split; intros; lia. }
+	          -- split.
+	             ++ unfold low_src in Hsrc |- *.
+	             destruct Hsrc as [Hsrc | [(v & Hdone_v & Hdg_v & Hfa_v & Hfa_neq_v & Hlow_v) |
+	                                      (w & Hdone_w & Hdg_w & Hstack_w & Hfa_neq_w & Hlow_w)]].
+	             ** left. exact Hsrc.
+	             ** right. left. exists v. repeat split; auto. sets_unfold. left. exact Hdone_v.
+	             ** right. right. exists w. repeat split; auto. sets_unfold. left. exact Hdone_w.
+	             ++ split.
+	                ** unfold children_low_valid in Hchild |- *.
+	                intros v Hv_done Hv_dg Hfa_v Hfa_neq_v.
+	                sets_unfold in Hv_done. destruct Hv_done as [Hv_done | Hv_eq].
+	                --- apply Hchild; auto.
+	                --- subst v. exact Hvalid_a.
+	                ** split.
+	                   --- exact Hfa_child.
+	                   --- exact Hfa_not.
   Qed.
 
   Lemma low_continuation_contract_from_tree_child_frame
@@ -2099,13 +2561,15 @@ Section IS_LOW.
       (Q := fun _ s => low_tree_child_after_set_fa u a done s).
     - eapply Hoare_conseq_post.
       2: {
-        apply Hoare_conj with
-          (Q1 := fun _ s =>
-             wf_scc_state_pre g root a s /\
-             u ∈ visited s /\
-             In u (stack s) /\
-             done_visited done s /\
-             low_frontier g u done s /\
+	        apply Hoare_conj with
+	          (Q1 := fun _ s =>
+	             wf_scc_state_pre g root a s /\
+	             settled_closed g s /\
+	             u ∈ visited s /\
+	             In u (stack s) /\
+	             done_visited done s /\
+	             done_reachable_closed g done s /\
+	             low_frontier g u done s /\
 	             low_src g u done s /\
 	             children_low_valid g root u done s /\
 	             fa_child_of_u g u s /\
@@ -2133,15 +2597,18 @@ Section IS_LOW.
 	              2: { apply (set_fa_keep_dfn_injective a u). }
 	              intros st [Heq [Hiter [Hord [Hinj Hnvis]]]]. exact Hinj. }
 	      intros r st [Hset [Hfa_not_pending [Hord Hinj]]].
-      unfold low_tree_child_after_set_fa.
-      destruct Hset as
-        (Hwfpre & Huvis & Hustack & Hdonevis & Hfront & Hsrc &
-         Hchild & Hfa_child & Hfa_a).
-      split; [exact Hwfpre |].
-      split; [exact Huvis |].
-      split; [exact Hustack |].
-      split; [exact Hdonevis |].
-      split; [exact Hfront |].
+	      unfold low_tree_child_after_set_fa.
+	      destruct Hset as
+	        (Hwfpre & Hsettled & Huvis & Hustack & Hdonevis & Hclosed &
+           Hfront & Hsrc &
+	         Hchild & Hfa_child & Hfa_a).
+	      split; [exact Hwfpre |].
+	      split; [exact Hsettled |].
+	      split; [exact Huvis |].
+	      split; [exact Hustack |].
+	      split; [exact Hdonevis |].
+	      split; [exact Hclosed |].
+	      split; [exact Hfront |].
 	      split; [exact Hsrc |].
 	      split; [exact Hchild |].
 	      split; [exact Hfa_child |].
@@ -2177,6 +2644,61 @@ Section IS_LOW.
             (W a)
             (fun _ s => low_tree_child_parent_pending u a done s).
 
+  Definition low_parent_pending_frame_contract
+             (W: V -> program (@SCCSt V) unit): Prop :=
+    forall u a done parent x inner_done,
+      ~ done parent ->
+      dg_step g parent x ->
+      ~ inner_done x ->
+      Hoare (fun s =>
+               low_tree_child_parent_pending u a done s /\
+               low_tree_child_after_set_fa parent x inner_done s)
+            (W x)
+            (fun _ s => low_tree_child_parent_pending u a done s).
+
+  Lemma low_tree_child_after_set_fa_low_pre_with_frame
+        (u a parent x: V) (done inner_done: V -> Prop) (s: @SCCSt V):
+    low_tree_child_parent_pending u a done s ->
+    low_tree_child_after_set_fa parent x inner_done s ->
+    low_pre g root x s /\
+    settled_closed g s /\
+    stack_dfn_order s /\
+    dfn_injective s.
+  Proof.
+    intros _Hpending Hset.
+    unfold low_tree_child_after_set_fa in Hset.
+    destruct Hset as
+      (Hwfpre & Hsettled & _Hparent_vis & _Hparent_stack &
+       _Hdonevis & _Hclosed & _Hfront & _Hsrc & _Hchild &
+       _Hfa_child & _Hfa_not & _Hfa_x & Hord & Hinj).
+    split; [exact Hwfpre | split; [exact Hsettled | split; [exact Hord | exact Hinj]]].
+  Qed.
+
+  Lemma low_tree_child_after_set_fa_not_outer_done
+        (u a parent x: V) (done inner_done: V -> Prop) (s: @SCCSt V):
+    low_tree_child_parent_pending u a done s ->
+    low_tree_child_after_set_fa parent x inner_done s ->
+    ~ done x.
+  Proof.
+    intros Hpending Hset Hdone_x.
+    unfold low_tree_child_parent_pending in Hpending.
+    destruct Hpending as
+      (_Hwf & _Hsettled & _Huvis & _Hustack & Hdonevis & _).
+    unfold low_tree_child_after_set_fa in Hset.
+    destruct Hset as (Hwfpre & _).
+    unfold wf_scc_state_pre in Hwfpre.
+    destruct Hwfpre as [_Hwf_inner Hnot_x_vis].
+    apply Hnot_x_vis.
+    apply Hdonevis. exact Hdone_x.
+  Qed.
+
+  Inductive low_fix_mode: Type :=
+  | LowRootMode
+  | LowTreeChildMode (parent: V) (done: V -> Prop)
+  | LowParentPendingMode
+      (outer_parent outer_child: V) (outer_done: V -> Prop)
+      (direct_parent: V) (direct_done: V -> Prop).
+
   Lemma low_tree_child_after_set_fa_low_pre
         (u a: V) (done: V -> Prop) (s: @SCCSt V):
     low_tree_child_after_set_fa u a done s ->
@@ -2193,8 +2715,9 @@ Section IS_LOW.
     active_base ((u, s) :: nil) s.
   Proof.
     unfold low_tree_child_after_set_fa, active_base, active_stack_frames.
-    intros (Hwfpre & _Huvis & Hustack & _Hdonevis & _Hfront & _Hsrc &
-            _Hchild & _Hfa_child & _Hfa_not & _Hfa_a & Hord & Hinj).
+    intros (Hwfpre & _Hsettled & _Huvis & Hustack & _Hdonevis &
+            _Hclosed & _Hfront & _Hsrc & _Hchild & _Hfa_child &
+            _Hfa_not & _Hfa_a & Hord & Hinj).
     unfold wf_scc_state_pre in Hwfpre.
     destruct Hwfpre as [Hwf _Hnot_a].
     split.
@@ -2212,7 +2735,7 @@ Section IS_LOW.
     active_stack_frames_below_timer ((u, s) :: nil) s.
   Proof.
     unfold low_tree_child_after_set_fa, active_stack_frames_below_timer.
-    intros (Hwfpre & Huvis & _).
+    intros (Hwfpre & _Hsettled & Huvis & _).
     unfold wf_scc_state_pre, wf_scc_state in Hwfpre.
     destruct Hwfpre as [[_ [Hinv _]] _].
     destruct Hinv as [Htimer_lt _].
@@ -2297,10 +2820,10 @@ Section IS_LOW.
         (P2 := fun s => done_visited done s)
         (Q2 := fun _ s => forall v, done v -> v ∈ visited s).
     - intros st [Heq Hset].
-      subst st.
-      unfold low_tree_child_after_set_fa in Hset.
-      destruct Hset as (_ & _ & _ & Hdonevis & _).
-      exact Hdonevis.
+	      subst st.
+	      unfold low_tree_child_after_set_fa in Hset.
+	      destruct Hset as (_ & _ & _ & _ & Hdonevis & _).
+	      exact Hdonevis.
     - intros _ st Hdonevis.
       unfold done_visited.
       exact Hdonevis.
@@ -2316,10 +2839,11 @@ Section IS_LOW.
     unfold Hoare.
     intros s1 r s2 [Heq Hset] Hrun.
     subst s1.
-    unfold low_tree_child_after_set_fa in Hset.
-    destruct Hset as
-      (Hwfpre & Huvis & _Hustack & _Hdonevis & _Hfront & _Hsrc &
-       _Hchild & _Hfa_child & _Hfa_not & Hfa_a & _Hord & _Hinj).
+	    unfold low_tree_child_after_set_fa in Hset.
+	    destruct Hset as
+	      (Hwfpre & _Hsettled & Huvis & _Hustack & _Hdonevis & _Hclosed &
+	       _Hfront & _Hsrc & _Hchild & _Hfa_child & _Hfa_not & Hfa_a &
+         _Hord & _Hinj).
     unfold wf_scc_state_pre in Hwfpre.
     destruct Hwfpre as [_Hwf Hnot_a_vis].
     assert (Ha_neq_u: a <> u).
@@ -2345,9 +2869,11 @@ Section IS_LOW.
   Lemma low_tree_child_parent_pending_from_fields
         (u a: V) (done: V -> Prop) (s: @SCCSt V):
     wf_scc_state g root s ->
+    settled_closed g s ->
     u ∈ visited s ->
     In u (stack s) ->
     done_visited done s ->
+    done_reachable_closed g done s ->
     low_tree_child_parent_low_fields u a done s ->
     stack_dfn_order s ->
     dfn_injective s ->
@@ -2358,14 +2884,16 @@ Section IS_LOW.
     fa s a <> a ->
     low_tree_child_parent_pending u a done s.
   Proof.
-    intros Hwf Huvis Hustack Hdonevis Hfields Hord Hinj
-           Hdg Hndone Hvis_a Hfa_a Hfa_neq_a.
+    intros Hwf Hsettled Huvis Hustack Hdonevis Hclosed Hfields Hord Hinj
+	           Hdg Hndone Hvis_a Hfa_a Hfa_neq_a.
     destruct Hfields as [Hfront [Hsrc [Hchild [Hfa_child Hfa_not]]]].
     unfold low_tree_child_parent_pending.
     split; [exact Hwf |].
+    split; [exact Hsettled |].
     split; [exact Huvis |].
     split; [exact Hustack |].
     split; [exact Hdonevis |].
+    split; [exact Hclosed |].
     split; [exact Hfront |].
     split; [exact Hsrc |].
     split; [exact Hchild |].
@@ -2377,6 +2905,944 @@ Section IS_LOW.
     split; [exact Hndone |].
     split; [exact Hvis_a |].
     split; [exact Hfa_a | exact Hfa_neq_a].
+  Qed.
+
+  Definition preloop_state (u: V) (s: @SCCSt V): @SCCSt V :=
+    RecordSet.set visited (fun vis => vis ∪ [u])
+      (RecordSet.set stack (fun stk => u :: stk)
+        (RecordSet.set timer (fun t => S t)
+          (RecordSet.set low
+            (fun low0 x => if equiv_decb x u then timer s else low0 x)
+            (RecordSet.set dfn
+              (fun dfn0 x => if equiv_decb x u then timer s else dfn0 x)
+              s)))).
+
+  Lemma preloop_exact_state (u: V) (s0: @SCCSt V):
+    Hoare (fun s: @SCCSt V => s = s0)
+          (preloop u)
+          (fun _ s => s = preloop_state u s0).
+  Proof.
+    unfold preloop, preloop_state. unfold_op.
+    intro_state. hoare_auto_s.
+  Qed.
+
+  Lemma preloop_state_visited_iff
+        (u v: V) (s: @SCCSt V):
+    v ∈ visited (preloop_state u s) <-> v ∈ visited s \/ v = u.
+  Proof.
+    unfold preloop_state. simpl. sets_unfold.
+    split; intros H.
+    - destruct H as [Hv | Hv].
+      + left. exact Hv.
+      + right. symmetry. exact Hv.
+    - destruct H as [Hv | Hv].
+      + left. exact Hv.
+      + right. symmetry. exact Hv.
+  Qed.
+
+  Lemma preloop_state_stack_iff
+        (u v: V) (s: @SCCSt V):
+    In v (stack (preloop_state u s)) <-> v = u \/ In v (stack s).
+  Proof.
+    unfold preloop_state. simpl.
+    split; intros H.
+    - destruct H as [Hv | Hv].
+      + left. symmetry. exact Hv.
+      + right. exact Hv.
+    - destruct H as [Hv | Hv].
+      + left. symmetry. exact Hv.
+      + right. exact Hv.
+  Qed.
+
+  Lemma preloop_state_fa
+        (u v: V) (s: @SCCSt V):
+    fa (preloop_state u s) v = fa s v.
+  Proof.
+    unfold preloop_state. simpl. reflexivity.
+  Qed.
+
+  Lemma preloop_state_dfn_eq
+        (u: V) (s: @SCCSt V):
+    dfn (preloop_state u s) u = timer s.
+  Proof.
+    unfold preloop_state. simpl. unfold equiv_decb.
+    destruct (equiv_dec u u) as [_ | Hneq].
+    - reflexivity.
+    - exfalso. apply Hneq. reflexivity.
+  Qed.
+
+  Lemma preloop_state_dfn_neq
+        (u v: V) (s: @SCCSt V):
+    v <> u ->
+    dfn (preloop_state u s) v = dfn s v.
+  Proof.
+    intros Hneq.
+    unfold preloop_state. simpl. unfold equiv_decb.
+    destruct (equiv_dec v u) as [Heq | _].
+    - contradiction.
+    - reflexivity.
+  Qed.
+
+  Lemma preloop_state_low_eq
+        (u: V) (s: @SCCSt V):
+    low (preloop_state u s) u = timer s.
+  Proof.
+    unfold preloop_state. simpl. unfold equiv_decb.
+    destruct (equiv_dec u u) as [_ | Hneq].
+    - reflexivity.
+    - exfalso. apply Hneq. reflexivity.
+  Qed.
+
+  Lemma preloop_state_low_neq
+        (u v: V) (s: @SCCSt V):
+    v <> u ->
+    low (preloop_state u s) v = low s v.
+  Proof.
+    intros Hneq.
+    unfold preloop_state. simpl. unfold equiv_decb.
+    destruct (equiv_dec v u) as [Heq | _].
+    - contradiction.
+    - reflexivity.
+  Qed.
+
+  Lemma preloop_state_tree_step_old
+        (u x y: V) (s: @SCCSt V):
+    y <> u ->
+    dg_step (state_to_dfs_tree g (preloop_state u s) root) x y ->
+    dg_step (state_to_dfs_tree g s root) x y.
+  Proof.
+    intros Hy_ne_u Hstep.
+    unfold dg_step in Hstep |- *.
+    destruct Hstep as [e [Horig [Hfst Hsnd]]].
+    exists e. split; [| split; [exact Hfst | exact Hsnd]].
+    unfold state_to_dfs_tree, original_step in Horig |- *.
+    simpl in Horig, Hfst, Hsnd |- *.
+    destruct Horig as [v [Hvis [Hfa_ne [Hfst_fa Hsnd_v]]]].
+    exists v. split.
+    - apply preloop_state_visited_iff in Hvis.
+      destruct Hvis as [Hvis | Hv_eq_u].
+      + exact Hvis.
+      + exfalso. apply Hy_ne_u.
+        assert (Hv_y: v = y) by congruence.
+        rewrite <- Hv_y. exact Hv_eq_u.
+    - split; [exact Hfa_ne | split; [exact Hfst_fa | exact Hsnd_v]].
+  Qed.
+
+  Lemma preloop_state_tree_step_new
+        (u x y: V) (s: @SCCSt V):
+    dg_step (state_to_dfs_tree g s root) x y ->
+    dg_step (state_to_dfs_tree g (preloop_state u s) root) x y.
+  Proof.
+    intros Hstep.
+    unfold dg_step in Hstep |- *.
+    destruct Hstep as [e [Horig [Hfst Hsnd]]].
+    exists e. split; [| split; [exact Hfst | exact Hsnd]].
+    unfold state_to_dfs_tree, original_step in Horig |- *.
+    simpl in Horig, Hfst, Hsnd |- *.
+    destruct Horig as [v [Hvis [Hfa_ne [Hfst_fa Hsnd_v]]]].
+    exists v. split.
+    - apply preloop_state_visited_iff. left. exact Hvis.
+    - split; [exact Hfa_ne | split; [exact Hfst_fa | exact Hsnd_v]].
+  Qed.
+
+  Lemma preloop_state_not_tree_child_of_sibling
+        (u a v: V) (s: @SCCSt V):
+    fa s a = u ->
+    v <> u ->
+    ~ dg_step (state_to_dfs_tree g (preloop_state a s) root) v a.
+  Proof.
+    intros Hfa_a Hv_ne_u Htree.
+    apply tree_step_char in Htree.
+    destruct Htree as [Hfa_tree [_ _]].
+    rewrite preloop_state_fa in Hfa_tree.
+    congruence.
+  Qed.
+
+  Lemma preloop_state_back_edge_old_or_new
+        (a v y: V) (s: @SCCSt V):
+    scc_back_edge g root (preloop_state a s) v y ->
+    y = a \/ scc_back_edge g root s v y.
+  Proof.
+    unfold scc_back_edge.
+    intros [Hdg [Hstack Hnot_tree]].
+    apply preloop_state_stack_iff in Hstack.
+    destruct Hstack as [Hy_eq_a | Hstack_old].
+    - left. exact Hy_eq_a.
+    - right. split; [exact Hdg | split; [exact Hstack_old |]].
+      intro Htree_old.
+      apply Hnot_tree.
+      apply preloop_state_tree_step_new. exact Htree_old.
+  Qed.
+
+  Lemma scc_low_valid_v_bound_tree_child
+        (s: @SCCSt V) (v w: V):
+    scc_low_valid_v g root s v ->
+    dg_step (state_to_dfs_tree g s root) v w ->
+    low s v <= low s w.
+  Proof.
+    unfold scc_low_valid_v, min_value_of_subset, min_object_of_subset.
+    intros [m [[Hm_src Hm_min] Hm_eq]] Htree.
+    rewrite <- Hm_eq.
+    pose proof (min_nonempty_exists
+                  (fun x => low s x)
+                  (dg_step (state_to_dfs_tree g s root) v)) as Hmin.
+    destruct Hmin as [m_child Hm_child].
+    { exists w. exact Htree. }
+    eapply Nat.le_trans.
+    - apply Hm_min. left. exact Hm_child.
+    - destruct Hm_child as [child [[_ Hchild_min] Hchild_eq]].
+      rewrite <- Hchild_eq.
+      apply Hchild_min. exact Htree.
+  Qed.
+
+  Lemma scc_low_valid_v_bound_back_edge
+        (s: @SCCSt V) (v w: V):
+    scc_low_valid_v g root s v ->
+    scc_back_edge g root s v w ->
+    low s v <= dfn s w.
+  Proof.
+    unfold scc_low_valid_v, min_value_of_subset, min_object_of_subset.
+    intros [m [[Hm_src Hm_min] Hm_eq]] Hback.
+    rewrite <- Hm_eq.
+    pose proof (min_nonempty_exists
+                  (fun x => dfn s x)
+                  (scc_back_edge g root s v ∪ [v])) as Hmin.
+    destruct Hmin as [m_back Hm_back].
+    { exists w. sets_unfold. left. exact Hback. }
+    eapply Nat.le_trans.
+    - apply Hm_min. right. exact Hm_back.
+    - destruct Hm_back as [back [[_ Hback_min] Hback_eq]].
+      rewrite <- Hback_eq.
+      apply Hback_min. sets_unfold. left. exact Hback.
+  Qed.
+
+  Lemma preloop_state_old_back_edge_new
+        (a v y: V) (s: @SCCSt V):
+    wf_scc_state g root s ->
+    ~ a ∈ visited s ->
+    scc_back_edge g root s v y ->
+    scc_back_edge g root (preloop_state a s) v y.
+  Proof.
+    intros Hwf Hnot_a_vis Hback.
+    unfold scc_back_edge in Hback |- *.
+    destruct Hback as [Hdg [Hstack Hnot_tree]].
+    destruct Hwf as [Hstack_in _].
+    assert (Hy_ne_a: y <> a).
+    { intro Hy_eq_a. subst y. apply Hnot_a_vis. apply Hstack_in. exact Hstack. }
+    split; [exact Hdg | split; [|]].
+    - apply preloop_state_stack_iff. right. exact Hstack.
+    - intro Htree_new.
+      apply Hnot_tree.
+      eapply preloop_state_tree_step_old; eauto.
+  Qed.
+
+  Lemma preloop_state_preserves_scc_low_valid_for_sibling
+        (u a v: V) (s: @SCCSt V):
+    wf_scc_state g root s ->
+    v ∈ visited s ->
+    fa s v = u ->
+    fa s v <> v ->
+    fa s a = u ->
+    ~ a ∈ visited s ->
+    scc_low_valid_v g root s v ->
+    scc_low_valid_v g root (preloop_state a s) v.
+  Proof.
+    intros Hwf Hvis_v Hfa_v Hfa_v_ne Hfa_a Hnot_a_vis Hvalid.
+    pose proof Hwf as Hwf_all.
+    pose proof Hvalid as Hvalid_all.
+    assert (Hv_ne_a: v <> a).
+    { intro Hv_eq_a. subst v. apply Hnot_a_vis. exact Hvis_v. }
+    assert (Hv_ne_u: v <> u).
+    { intro Hv_eq_u. apply Hfa_v_ne. rewrite Hfa_v. symmetry. exact Hv_eq_u. }
+    destruct Hwf as [Hstack_in [Hdfn_inv Hwf_tail]].
+    destruct Hdfn_inv as [Hdfn_lt _].
+    unfold scc_low_valid_v, min_value_of_subset, min_object_of_subset in *.
+    destruct Hvalid as [m [[Hm_src Hm_min] Hm_eq]].
+    exists m. split.
+    - split.
+      + destruct Hm_src as [Hm_child | Hm_back].
+        * left.
+          destruct Hm_child as [x [[Htree_x Hmin_x] Hx_eq]].
+          assert (Hx_ne_a: x <> a).
+          { intro Hx_eq_a.
+            subst x.
+            apply tree_step_char in Htree_x as [_ [_ Hx_vis]].
+            apply Hnot_a_vis. exact Hx_vis. }
+          exists x. split.
+          -- split.
+             ++ apply preloop_state_tree_step_new. exact Htree_x.
+             ++ intros y Htree_y_new.
+                assert (Hy_ne_a: y <> a).
+                { intro Hy_eq_a.
+                  subst y.
+                  eapply preloop_state_not_tree_child_of_sibling; eauto. }
+                rewrite preloop_state_low_neq by exact Hx_ne_a.
+                rewrite preloop_state_low_neq by exact Hy_ne_a.
+                apply Hmin_x.
+                eapply preloop_state_tree_step_old; eauto.
+          -- rewrite preloop_state_low_neq by exact Hx_ne_a.
+             exact Hx_eq.
+        * right.
+          destruct Hm_back as [x [[Hx Hmin_x] Hx_eq]].
+          assert (Hx_ne_a: x <> a).
+          { sets_unfold in Hx.
+            destruct Hx as [Hback_x | Hx_eq_v].
+            - unfold scc_back_edge in Hback_x.
+              destruct Hback_x as [_ [Hstack_x _]].
+              intro Hx_eq_a. subst x.
+              apply Hnot_a_vis. apply Hstack_in. exact Hstack_x.
+            - subst x. exact Hv_ne_a. }
+          exists x. split.
+          -- split.
+             ++ sets_unfold in Hx. sets_unfold.
+                destruct Hx as [Hback_x | Hx_eq_v].
+                ** left.
+                   eapply preloop_state_old_back_edge_new; eauto.
+                ** right. exact Hx_eq_v.
+             ++ intros y Hy.
+                rewrite preloop_state_dfn_neq by exact Hx_ne_a.
+                sets_unfold in Hy.
+                destruct Hy as [Hback_y_new | Hy_eq_v].
+                ** pose proof (preloop_state_back_edge_old_or_new a v y s Hback_y_new)
+                     as [Hy_eq_a | Hback_y_old].
+                   --- subst y.
+                       rewrite preloop_state_dfn_eq.
+                       eapply Nat.le_trans.
+                       { apply Hmin_x. sets_unfold. right. reflexivity. }
+                       { apply Nat.lt_le_incl. apply Hdfn_lt. exact Hvis_v. }
+                   --- assert (Hy_ne_a: y <> a).
+                       { unfold scc_back_edge in Hback_y_old.
+                         destruct Hback_y_old as [_ [Hstack_y _]].
+                         intro Hy_eq_a. subst y.
+                         apply Hnot_a_vis. apply Hstack_in. exact Hstack_y. }
+                       rewrite preloop_state_dfn_neq by exact Hy_ne_a.
+                       apply Hmin_x. sets_unfold. left. exact Hback_y_old.
+                ** subst y.
+                   rewrite preloop_state_dfn_neq by exact Hv_ne_a.
+                   apply Hmin_x. sets_unfold. right. reflexivity.
+          -- rewrite preloop_state_dfn_neq by exact Hx_ne_a.
+             exact Hx_eq.
+      + intros n Hn.
+        rewrite Hm_eq.
+        destruct Hn as [Hn_child | Hn_back].
+        * destruct Hn_child as [x [[Htree_x_new _Hmin_x] Hx_eq]].
+          assert (Hx_ne_a: x <> a).
+          { intro Hx_eq_a.
+            subst x.
+            eapply preloop_state_not_tree_child_of_sibling; eauto. }
+          rewrite <- Hx_eq.
+          rewrite preloop_state_low_neq by exact Hx_ne_a.
+          apply scc_low_valid_v_bound_tree_child with (w := x) in Hvalid_all.
+          -- exact Hvalid_all.
+          -- eapply preloop_state_tree_step_old; eauto.
+        * destruct Hn_back as [x [[Hx _Hmin_x] Hx_eq]].
+          rewrite <- Hx_eq.
+          sets_unfold in Hx.
+          destruct Hx as [Hback_x_new | Hx_eq_v].
+          -- pose proof (preloop_state_back_edge_old_or_new a v x s Hback_x_new)
+               as [Hx_eq_a | Hback_x_old].
+             ++ subst x.
+                rewrite preloop_state_dfn_eq.
+                eapply Nat.le_trans.
+                { apply (scc_low_valid_v_bound_self g root s v). exact Hvalid_all. }
+                { apply Nat.lt_le_incl. apply Hdfn_lt. exact Hvis_v. }
+             ++ assert (Hx_ne_a: x <> a).
+                { unfold scc_back_edge in Hback_x_old.
+                  destruct Hback_x_old as [_ [Hstack_x _]].
+                  intro Hx_eq_a. subst x.
+                  apply Hnot_a_vis. apply Hstack_in. exact Hstack_x. }
+                rewrite preloop_state_dfn_neq by exact Hx_ne_a.
+                apply scc_low_valid_v_bound_back_edge with (w := x) in Hvalid_all.
+                ** exact Hvalid_all.
+                ** exact Hback_x_old.
+          -- subst x.
+             rewrite preloop_state_dfn_neq by exact Hv_ne_a.
+             apply (scc_low_valid_v_bound_self g root s v). exact Hvalid_all.
+    - rewrite preloop_state_low_neq by exact Hv_ne_a.
+      exact Hm_eq.
+  Qed.
+
+  Lemma preloop_establishes_parent_pending_from_after_set_fa
+        (u a: V) (done: V -> Prop):
+    dg_step g u a ->
+    ~ done a ->
+    Hoare (low_tree_child_after_set_fa u a done)
+          (preloop a)
+          (fun _ s => low_tree_child_parent_pending u a done s).
+  Proof.
+    intros Hdg Hndone.
+    apply Hoare_normalize. intros snap Hset.
+    eapply Hoare_conseq_post.
+    2: {
+      apply Hoare_conj with
+        (Q1 := fun _ s => s = preloop_state a snap)
+        (Q2 := fun _ s =>
+                 wf_scc_state g root s /\
+                 settled_closed g s /\
+                 stack_dfn_order s /\
+                 dfn_injective s).
+      - eapply Hoare_conseq_pre.
+        2: { apply (preloop_exact_state a snap). }
+        intros st Heq. exact Heq.
+      - apply Hoare_conj with
+          (Q1 := fun _ s => wf_scc_state g root s)
+          (Q2 := fun _ s =>
+                   settled_closed g s /\
+                   stack_dfn_order s /\
+                   dfn_injective s).
+        + eapply Hoare_conseq_pre.
+          2: { apply (preloop_preserves_wf_scc_state g root a). }
+          intros st Heq. subst st.
+          unfold low_tree_child_after_set_fa in Hset. tauto.
+        + apply Hoare_conj with
+            (Q1 := fun _ s => settled_closed g s)
+            (Q2 := fun _ s => stack_dfn_order s /\ dfn_injective s).
+          * eapply Hoare_conseq_pre.
+            2: { apply (preloop_keep_settled_closed g a). }
+            intros st Heq. subst st.
+            unfold low_tree_child_after_set_fa in Hset. tauto.
+          * apply Hoare_conj.
+            -- eapply Hoare_conseq_pre.
+               2: { apply (preloop_preserves_stack_dfn_order a). }
+               intros st Heq. subst st.
+               unfold low_tree_child_after_set_fa in Hset.
+               destruct Hset as (Hwfpre & _ & _ & _ & _ & _ & _ & _ &
+                                 _ & _ & _ & _ & Hord & _).
+	               unfold wf_scc_state_pre in Hwfpre.
+	               destruct Hwfpre as [Hwf Hnot_a].
+	               unfold wf_scc_state in Hwf.
+	               destruct Hwf as [Hsiv [Hinv _]].
+	               split; [exact Hord | split; [exact Hinv | split; [exact Hsiv | exact Hnot_a]]].
+            -- eapply Hoare_conseq_pre.
+               2: { apply (preloop_preserves_dfn_injective a). }
+               intros st Heq. subst st.
+               unfold low_tree_child_after_set_fa in Hset.
+               destruct Hset as (Hwfpre & _ & _ & _ & _ & _ & _ & _ &
+                                 _ & _ & _ & _ & _ & Hinj).
+	               unfold wf_scc_state_pre in Hwfpre.
+	               destruct Hwfpre as [Hwf Hnot_a].
+	               unfold wf_scc_state in Hwf.
+	               destruct Hwf as [_ [Hinv _]].
+	               split; [exact Hinj | split; [exact Hinv | exact Hnot_a]]. }
+    intros _ st [Heq_state [Hwf_post [Hsettled_post [Hord_post Hinj_post]]]].
+    subst st.
+    unfold low_tree_child_after_set_fa in Hset.
+    destruct Hset as
+      (Hwfpre & _Hsettled & Huvis & Hustack & Hdonevis & Hclosed &
+       Hfront & Hsrc & Hchild & Hfa_child & Hfa_not & Hfa_a &
+       _Hord & _Hinj).
+    unfold wf_scc_state_pre in Hwfpre.
+    destruct Hwfpre as [Hwf_old Hnot_a_vis].
+    assert (Ha_ne_u: a <> u).
+    { intro Ha_eq_u. subst a. apply Hnot_a_vis. exact Huvis. }
+    assert (Hu_ne_a: u <> a) by (intro Hu_eq_a; apply Ha_ne_u; symmetry; exact Hu_eq_a).
+    apply low_tree_child_parent_pending_from_fields.
+    - exact Hwf_post.
+    - exact Hsettled_post.
+    - apply preloop_state_visited_iff. left. exact Huvis.
+    - apply preloop_state_stack_iff. right. exact Hustack.
+    - unfold done_visited in Hdonevis |- *.
+      intros w Hdone_w.
+      apply preloop_state_visited_iff. left. apply Hdonevis. exact Hdone_w.
+    - unfold done_reachable_closed in Hclosed |- *.
+      intros v w Hdone_v Hnot_stack_v Hreach.
+      apply preloop_state_visited_iff. left.
+      eapply Hclosed; eauto.
+      intro Hstack_old. apply Hnot_stack_v.
+      apply preloop_state_stack_iff. right. exact Hstack_old.
+    - unfold low_tree_child_parent_low_fields.
+      split.
+      + unfold low_frontier in Hfront |- *.
+        destruct Hfront as [Hlow_dfn Hfront].
+        split.
+        * rewrite preloop_state_low_neq by exact Hu_ne_a.
+          rewrite preloop_state_dfn_neq by exact Hu_ne_a.
+          exact Hlow_dfn.
+        * intros v Hdone_v Hdg_v.
+          assert (Hv_ne_a: v <> a).
+          { intro Hv_eq_a. subst v. exact (Hndone Hdone_v). }
+          specialize (Hfront v Hdone_v Hdg_v) as [Hfa_part Hstack_part].
+          split.
+          -- intro Hfa_v.
+             rewrite preloop_state_fa in Hfa_v.
+             rewrite preloop_state_low_neq by exact Hu_ne_a.
+             rewrite preloop_state_low_neq by exact Hv_ne_a.
+             apply Hfa_part. exact Hfa_v.
+          -- intro Hstack_v.
+             apply preloop_state_stack_iff in Hstack_v.
+             destruct Hstack_v as [Hv_eq_a | Hstack_old].
+             { subst v. contradiction. }
+             rewrite preloop_state_low_neq by exact Hu_ne_a.
+             rewrite preloop_state_dfn_neq by exact Hv_ne_a.
+             apply Hstack_part. exact Hstack_old.
+      + split.
+        * unfold low_src in Hsrc |- *.
+          destruct Hsrc as [Hsrc | [(v & Hdone_v & Hdg_v & Hfa_v & Hfa_ne_v & Hlow_v) |
+                                   (w & Hdone_w & Hdg_w & Hstack_w & Hfa_ne_w & Hlow_w)]].
+          -- left.
+             rewrite preloop_state_low_neq by exact Hu_ne_a.
+             rewrite preloop_state_dfn_neq by exact Hu_ne_a.
+             exact Hsrc.
+	          -- right. left. exists v.
+	             assert (Hv_ne_a: v <> a).
+	             { intro Hv_eq_a. subst v. exact (Hndone Hdone_v). }
+	             split; [exact Hdone_v |].
+	             split; [exact Hdg_v |].
+	             split.
+	             ++ rewrite preloop_state_fa. exact Hfa_v.
+	             ++ split.
+	                ** rewrite preloop_state_fa. exact Hfa_ne_v.
+	                ** rewrite preloop_state_low_neq by exact Hu_ne_a.
+	                   rewrite preloop_state_low_neq by exact Hv_ne_a.
+	                   exact Hlow_v.
+	          -- right. right. exists w.
+	             assert (Hw_ne_a: w <> a).
+	             { intro Hw_eq_a. subst w. exact (Hndone Hdone_w). }
+	             split; [exact Hdone_w |].
+	             split; [exact Hdg_w |].
+	             split.
+	             ++ apply preloop_state_stack_iff. right. exact Hstack_w.
+	             ++ split.
+	                ** rewrite preloop_state_fa. exact Hfa_ne_w.
+	                ** rewrite preloop_state_low_neq by exact Hu_ne_a.
+	                   rewrite preloop_state_dfn_neq by exact Hw_ne_a.
+	                   exact Hlow_w.
+        * split.
+          -- unfold children_low_valid in Hchild |- *.
+             intros v Hdone_v Hdg_v Hfa_v Hfa_ne_v.
+             assert (Hv_vis: v ∈ visited snap).
+             { apply Hdonevis. exact Hdone_v. }
+             assert (Hv_ne_a: v <> a).
+             { intro Hv_eq_a. subst v. exact (Hndone Hdone_v). }
+	             rewrite preloop_state_fa in Hfa_v, Hfa_ne_v.
+	             apply preloop_state_preserves_scc_low_valid_for_sibling
+	               with (u := u); auto.
+	          -- split.
+             ++ unfold fa_child_of_u in Hfa_child |- *.
+                intros v [Hfa_v Hfa_ne_v].
+                apply Hfa_child.
+                rewrite preloop_state_fa in Hfa_v, Hfa_ne_v.
+                split; auto.
+             ++ unfold fa_not_done_implies_eq_u in Hfa_not |- *.
+	                intros v Hnot_done Hfa_v.
+	                apply Hfa_not; auto.
+    - exact Hord_post.
+    - exact Hinj_post.
+    - exact Hdg.
+    - exact Hndone.
+    - apply preloop_state_visited_iff. right. reflexivity.
+    - rewrite preloop_state_fa. exact Hfa_a.
+    - rewrite preloop_state_fa.
+      intro Hfa_loop.
+      apply Ha_ne_u.
+      rewrite <- Hfa_a.
+      symmetry; exact Hfa_loop.
+  Qed.
+
+  Lemma low_tree_child_parent_pending_not_tree_child_current
+        (u a: V) (done: V -> Prop) (s: @SCCSt V):
+    low_tree_child_parent_pending u a done s ->
+    forall v,
+      done v ->
+      dg_step g u v ->
+      fa s v = u ->
+      fa s v <> v ->
+      ~ dg_step (state_to_dfs_tree g s root) v a.
+  Proof.
+    intros Hpending v _Hdone_v _Hdg_v Hfa_v Hfa_ne_v Htree.
+    unfold low_tree_child_parent_pending in Hpending.
+    destruct Hpending as
+      (_Hwf & _Hsettled & _Huvis & _Hustack & _Hdonevis & _Hclosed &
+       _Hfront & _Hsrc & _Hchild & _Hfa_child & _Hfa_not & _Hord &
+       _Hinj & _Hdg & _Hndone & _Hvis_a & Hfa_a & _Hfa_ne_a).
+    apply tree_step_char in Htree.
+    destruct Htree as [Hfa_tree _].
+    assert (Hv_eq_u: v = u).
+    { rewrite <- Hfa_tree. exact Hfa_a. }
+    apply Hfa_ne_v.
+    rewrite Hv_eq_u in Hfa_v.
+    rewrite Hv_eq_u.
+    exact Hfa_v.
+  Qed.
+
+  Lemma update_low_child_preserves_parent_pending
+        (u a: V) (done: V -> Prop) (n: nat):
+    a <> u ->
+    ~ done a ->
+    Hoare (low_tree_child_parent_pending u a done)
+          (update_low a n)
+          (fun _ s => low_tree_child_parent_pending u a done s).
+  Proof.
+    intros Ha_ne_u Hndone.
+    unfold update_low. unfold_op. intro_state; hoare_auto_s.
+    - pose proof H as Hpending_all.
+      subst s. unfold RecordSet.set. simpl.
+      unfold low_tree_child_parent_pending in H.
+      destruct H as
+        (Hwf & Hsettled & Huvis & Hustack & Hdonevis & Hclosed &
+         Hfront & Hsrc & Hchild & Hfa_child & Hfa_not & Hord & Hinj &
+         Hdg & Hndone_a & Hvis_a & Hfa_a & Hfa_ne_a).
+      unfold low_tree_child_parent_pending.
+      split.
+      { unfold wf_scc_state in Hwf |- *. simpl. exact Hwf. }
+      split; [exact Hsettled |].
+      split; [exact Huvis |].
+      split; [exact Hustack |].
+      split; [exact Hdonevis |].
+      split; [exact Hclosed |].
+      split.
+      + unfold low_frontier in Hfront |- *.
+        destruct Hfront as [Hle Hrest].
+        split.
+        * simpl. unfold equiv_decb.
+          destruct (equiv_dec u a) as [Heq | _].
+          -- exfalso. apply Ha_ne_u. symmetry. exact Heq.
+          -- exact Hle.
+        * intros v Hdone_v Hdg_v.
+          specialize (Hrest v Hdone_v Hdg_v) as [Hfa_part Hstack_part].
+          split.
+          -- intro Hfa_v.
+             simpl. unfold equiv_decb.
+             destruct (equiv_dec u a) as [Heq_ua | _].
+             ++ exfalso. apply Ha_ne_u. symmetry. exact Heq_ua.
+             ++ destruct (equiv_dec v a) as [Heq_va | _].
+                ** exfalso. apply Hndone. rewrite <- Heq_va. exact Hdone_v.
+                ** apply Hfa_part. exact Hfa_v.
+          -- intro Hstack_v.
+             simpl. unfold equiv_decb.
+             destruct (equiv_dec u a) as [Heq_ua | _].
+             ++ exfalso. apply Ha_ne_u. symmetry. exact Heq_ua.
+             ++ apply Hstack_part. exact Hstack_v.
+      + split.
+        * unfold low_src in Hsrc |- *.
+          destruct Hsrc as [Hlow_eq |
+            [(v & Hdone_v & Hdg_v & Hfa_v & Hfa_ne_v & Hlow_eq) |
+             (w & Hdone_w & Hdg_w & Hstack_w & Hfa_ne_w & Hlow_eq_w)]].
+          -- left. simpl. unfold equiv_decb.
+             destruct (equiv_dec u a) as [Heq | _].
+             ++ exfalso. apply Ha_ne_u. symmetry. exact Heq.
+             ++ exact Hlow_eq.
+          -- right. left. exists v.
+             split; [exact Hdone_v |].
+             split; [exact Hdg_v |].
+             split; [exact Hfa_v |].
+             split; [exact Hfa_ne_v |].
+             simpl. unfold equiv_decb.
+             destruct (equiv_dec u a) as [Heq_ua | _].
+             ++ exfalso. apply Ha_ne_u. symmetry. exact Heq_ua.
+             ++ destruct (equiv_dec v a) as [Heq_va | _].
+                ** exfalso. apply Hndone. rewrite <- Heq_va. exact Hdone_v.
+                ** exact Hlow_eq.
+          -- right. right. exists w.
+             split; [exact Hdone_w |].
+             split; [exact Hdg_w |].
+             split; [exact Hstack_w |].
+             split; [exact Hfa_ne_w |].
+             simpl. unfold equiv_decb.
+             destruct (equiv_dec u a) as [Heq_ua | _].
+             ++ exfalso. apply Ha_ne_u. symmetry. exact Heq_ua.
+             ++ exact Hlow_eq_w.
+        * split.
+          -- unfold children_low_valid in Hchild |- *.
+             intros v Hdone_v Hdg_v Hfa_v Hfa_ne_v.
+             simpl in Hfa_v, Hfa_ne_v.
+             apply (set_low_preserves_scc_low_valid_v_when_not_child
+                      g root v a n s0).
+             ++ intro Hv_eq_a. subst v. apply Hndone. exact Hdone_v.
+	             ++ apply (low_tree_child_parent_pending_not_tree_child_current
+	                         u a done s0 Hpending_all v Hdone_v Hdg_v Hfa_v Hfa_ne_v).
+	             ++ apply Hchild; [exact Hdone_v | exact Hdg_v | exact Hfa_v | exact Hfa_ne_v].
+          -- split; [exact Hfa_child |].
+             split; [exact Hfa_not |].
+             split; [exact Hord |].
+             split; [exact Hinj |].
+             split; [exact Hdg |].
+             split; [exact Hndone_a |].
+             split; [exact Hvis_a |].
+             split; [exact Hfa_a | exact Hfa_ne_a].
+    - destruct H1 as [Heq _]. subst s. exact H.
+  Qed.
+
+  Lemma get_low_update_low_child_preserves_parent_pending
+        (u a x: V) (done: V -> Prop):
+    a <> u ->
+    ~ done a ->
+    Hoare (low_tree_child_parent_pending u a done)
+          (lv <- get' (fun s => low s x);; update_low a lv)
+          (fun _ s => low_tree_child_parent_pending u a done s).
+  Proof.
+    intros Ha_ne_u Hndone.
+    apply Hoare_normalize. intros snap Hsnap.
+	    eapply Hoare_bind. { eapply Hoare_get'. } simpl. intros lv.
+	    eapply Hoare_conseq_pre.
+	    2: { exact (update_low_child_preserves_parent_pending
+                    u a done lv Ha_ne_u Hndone). }
+    intros st [Heq _]. subst st. exact Hsnap.
+  Qed.
+
+  Lemma get_dfn_update_low_child_preserves_parent_pending
+        (u a x: V) (done: V -> Prop):
+    a <> u ->
+    ~ done a ->
+    Hoare (low_tree_child_parent_pending u a done)
+          (dv <- get' (fun s => dfn s x);; update_low a dv)
+          (fun _ s => low_tree_child_parent_pending u a done s).
+  Proof.
+    intros Ha_ne_u Hndone.
+    apply Hoare_normalize. intros snap Hsnap.
+	    eapply Hoare_bind. { eapply Hoare_get'. } simpl. intros dv.
+	    eapply Hoare_conseq_pre.
+	    2: { exact (update_low_child_preserves_parent_pending
+                    u a done dv Ha_ne_u Hndone). }
+    intros st [Heq _]. subst st. exact Hsnap.
+  Qed.
+
+  Lemma set_fa_fresh_child_preserves_parent_pending
+        (u a x: V) (done: V -> Prop):
+    a <> u ->
+    Hoare (fun s: @SCCSt V =>
+             low_tree_child_parent_pending u a done s /\
+             ~ x ∈ visited s)
+          (set_fa x a)
+          (fun _ s => low_tree_child_parent_pending u a done s).
+  Proof.
+    intros Ha_ne_u.
+    unfold set_fa. intro_state; hoare_auto_s.
+    subst s. unfold RecordSet.set. simpl.
+    destruct H as [Hpending Hnot_x_vis].
+    pose proof Hpending as Hpending_all.
+    unfold low_tree_child_parent_pending in Hpending.
+    destruct Hpending as
+      (Hwf & Hsettled & Huvis & Hustack & Hdonevis & Hclosed &
+       Hfront & Hsrc & Hchild & Hfa_child & Hfa_not & Hord & Hinj &
+       Hdg & Hndone & Hvis_a & Hfa_a & Hfa_ne_a).
+    assert (Hx_ne_a: x <> a).
+    { intro Hx_eq_a. subst x. apply Hnot_x_vis. exact Hvis_a. }
+    unfold low_tree_child_parent_pending.
+    split.
+    { unfold wf_scc_state in Hwf |- *.
+      destruct Hwf as [Hsiv [Hinv [Hvalid Hfa_vis]]].
+      split; [exact Hsiv |].
+      split; [exact Hinv |].
+      split; [|].
+      - unfold dfn_valid in Hvalid |- *.
+        intros p q Htree.
+        apply Hvalid.
+        apply (proj1 (set_fa_unvisited_preserves_tree_step g root x a p q s0 Hnot_x_vis)).
+        exact Htree.
+	      - unfold fa_visited in Hfa_vis |- *.
+	        intros v Hfa_ne_v.
+	        simpl in Hfa_ne_v |- *.
+	        unfold equiv_decb in Hfa_ne_v |- *.
+	        destruct (equiv_dec v x) as [Hv_eq_x | Hv_ne_x].
+	        + exact Hvis_a.
+	        + apply Hfa_vis. exact Hfa_ne_v. }
+    split; [exact Hsettled |].
+    split; [exact Huvis |].
+    split; [exact Hustack |].
+    split; [exact Hdonevis |].
+    split; [exact Hclosed |].
+    split.
+    - unfold low_frontier in Hfront |- *.
+      destruct Hfront as [Hle Hrest].
+      split; [exact Hle |].
+      intros v Hdone_v Hdg_v.
+      assert (Hv_ne_x: v <> x).
+      { intro Hv_eq_x. subst v. apply Hnot_x_vis. apply Hdonevis. exact Hdone_v. }
+      specialize (Hrest v Hdone_v Hdg_v) as [Hfa_part Hstack_part].
+      split.
+      + intro Hfa_v.
+        simpl in Hfa_v. unfold equiv_decb in Hfa_v.
+        destruct (equiv_dec v x) as [Hv_eq_x | _].
+        * exfalso. apply Hv_ne_x. exact Hv_eq_x.
+        * apply Hfa_part. exact Hfa_v.
+      + intro Hstack_v. apply Hstack_part. exact Hstack_v.
+    - split.
+      + unfold low_src in Hsrc |- *.
+        destruct Hsrc as [Hsrc |
+          [(v & Hdone_v & Hdg_v & Hfa_v & Hfa_ne_v & Hlow_v) |
+           (w & Hdone_w & Hdg_w & Hstack_w & Hfa_ne_w & Hlow_w)]].
+        * left. exact Hsrc.
+        * right. left. exists v.
+          assert (Hv_ne_x: v <> x).
+          { intro Hv_eq_x. subst v. apply Hnot_x_vis. apply Hdonevis. exact Hdone_v. }
+          split; [exact Hdone_v |].
+          split; [exact Hdg_v |].
+          split.
+          -- simpl. unfold equiv_decb.
+             destruct (equiv_dec v x) as [Hv_eq_x | _].
+             ++ exfalso. apply Hv_ne_x. exact Hv_eq_x.
+             ++ exact Hfa_v.
+          -- split.
+             ++ simpl. unfold equiv_decb.
+                destruct (equiv_dec v x) as [Hv_eq_x | _].
+                ** exfalso. apply Hv_ne_x. exact Hv_eq_x.
+                ** exact Hfa_ne_v.
+             ++ exact Hlow_v.
+        * right. right. exists w.
+          assert (Hw_ne_x: w <> x).
+          { intro Hw_eq_x. subst w. apply Hnot_x_vis. apply Hdonevis. exact Hdone_w. }
+          split; [exact Hdone_w |].
+          split; [exact Hdg_w |].
+          split; [exact Hstack_w |].
+          split.
+          -- simpl. unfold equiv_decb.
+             destruct (equiv_dec w x) as [Hw_eq_x | _].
+             ++ exfalso. apply Hw_ne_x. exact Hw_eq_x.
+             ++ exact Hfa_ne_w.
+          -- exact Hlow_w.
+      + split.
+        * unfold children_low_valid in Hchild |- *.
+          intros v Hdone_v Hdg_v Hfa_v Hfa_ne_v.
+          assert (Hv_ne_x: v <> x).
+          { intro Hv_eq_x. subst v. apply Hnot_x_vis. apply Hdonevis. exact Hdone_v. }
+          simpl in Hfa_v, Hfa_ne_v. unfold equiv_decb in Hfa_v, Hfa_ne_v.
+          destruct (equiv_dec v x) as [Hv_eq_x | _].
+          { exfalso. apply Hv_ne_x. exact Hv_eq_x. }
+	          apply (set_fa_preserves_scc_low_valid_v_when_unvisited
+	                   g root v x a s0 Hnot_x_vis).
+	          apply Hchild; [exact Hdone_v | exact Hdg_v | exact Hfa_v | exact Hfa_ne_v].
+        * split.
+          -- unfold fa_child_of_u in Hfa_child |- *.
+             intros v [Hfa_v Hfa_ne_v].
+	             simpl in Hfa_v, Hfa_ne_v. unfold equiv_decb in Hfa_v, Hfa_ne_v.
+	             destruct (equiv_dec v x) as [Hv_eq_x | _].
+	             ++ exfalso. apply Ha_ne_u. exact Hfa_v.
+		             ++ apply Hfa_child. split; [exact Hfa_v | exact Hfa_ne_v].
+          -- split.
+             ++ unfold fa_not_done_implies_eq_u in Hfa_not |- *.
+                intros v Hnot_done Hfa_v.
+	                simpl in Hfa_v. unfold equiv_decb in Hfa_v.
+	                destruct (equiv_dec v x) as [Hv_eq_x | _].
+	                ** exfalso. apply Ha_ne_u. exact Hfa_v.
+		                ** apply Hfa_not; [exact Hnot_done | exact Hfa_v].
+             ++ split; [exact Hord |].
+                split; [exact Hinj |].
+                split; [exact Hdg |].
+                split; [exact Hndone |].
+                split; [exact Hvis_a |].
+                split.
+                ** simpl. unfold equiv_decb.
+                   destruct (equiv_dec a x) as [Ha_eq_x | _].
+                   --- exfalso. apply Hx_ne_a. symmetry. exact Ha_eq_x.
+                   --- exact Hfa_a.
+                ** simpl. unfold equiv_decb.
+                   destruct (equiv_dec a x) as [Ha_eq_x | _].
+                   --- exfalso. apply Hx_ne_a. symmetry. exact Ha_eq_x.
+                   --- exact Hfa_ne_a.
+  Qed.
+
+  Lemma process_edge_preserves_parent_pending
+        (W: V -> program (@SCCSt V) unit)
+        (u a x: V) (done inner_done: V -> Prop):
+    a <> u ->
+    ~ done a ->
+    low_parent_pending_frame_contract W ->
+    dg_step g a x ->
+    ~ inner_done x ->
+    Hoare (fun s =>
+             low_tree_child_parent_pending u a done s /\
+             low_iteration_inv g root a inner_done s /\
+             stack_dfn_order s /\
+             dfn_injective s /\
+             dg_step g a x /\
+             ~ inner_done x)
+          (process_edge a W x)
+          (fun _ s => low_tree_child_parent_pending u a done s).
+  Proof.
+    intros Ha_ne_u Houter_ndone Hparent_frame Hdg_ax Hinner_ndone.
+    unfold process_edge, if_else, If.
+    intro_state.
+    apply Hoare_choice.
+    - apply Hoare_assume_bind. simpl.
+      eapply Hoare_bind.
+      + apply Hoare_conj with
+          (Q1 := fun _ s => low_tree_child_parent_pending u a done s)
+          (Q2 := fun _ s => low_tree_child_after_set_fa a x inner_done s).
+        * eapply Hoare_conseq_pre.
+          2: { apply set_fa_fresh_child_preserves_parent_pending; exact Ha_ne_u. }
+          intros st [Hnot_vis Heq_st]. subst st.
+          split; [exact (proj1 H) | exact Hnot_vis].
+        * eapply Hoare_conseq_post.
+          2: {
+            apply Hoare_conj with
+              (Q1 := fun _ s =>
+                 wf_scc_state_pre g root x s /\
+                 settled_closed g s /\
+                 a ∈ visited s /\
+                 In a (stack s) /\
+                 done_visited inner_done s /\
+                 done_reachable_closed g inner_done s /\
+                 low_frontier g a inner_done s /\
+                 low_src g a inner_done s /\
+                 children_low_valid g root a inner_done s /\
+                 fa_child_of_u g a s /\
+                 fa s x = a)
+              (Q2 := fun _ s =>
+                 fa_not_done_implies_eq_u a (inner_done ∪ [x]) s /\
+                 stack_dfn_order s /\
+                 dfn_injective s).
+            - eapply Hoare_conseq_pre.
+              2: { apply (set_fa_establishes_low_iteration_before_new_child
+                            g root a x inner_done). }
+              intros st [Hnot_vis Heq_st]. subst st.
+              destruct H as [_ [Hiter [Hord [Hinj [_ _]]]]].
+              split; [exact Hiter |].
+              split; [exact Hnot_vis |].
+              split; [exact Hinner_ndone | exact Hdg_ax].
+            - apply Hoare_conj.
+              + eapply Hoare_conseq_pre.
+                2: { apply (set_fa_establishes_pending_fa_not_done a x inner_done). }
+                intros st [Hnot_vis Heq_st]. subst st.
+                destruct H as [_ [Hiter _]].
+                split; [exact Hiter | exact Hinner_ndone].
+              + apply Hoare_conj.
+                * eapply Hoare_conseq_pre.
+                  2: { apply (set_fa_keep_stack_dfn_order x a). }
+                  intros st [Hnot_vis Heq_st]. subst st.
+                  destruct H as [_ [_ [Hord _]]]. exact Hord.
+                * eapply Hoare_conseq_pre.
+                  2: { apply (set_fa_keep_dfn_injective x a). }
+                  intros st [Hnot_vis Heq_st]. subst st.
+                  destruct H as [_ [_ [_ [Hinj _]]]]. exact Hinj. }
+          intros _ st [Hset [Hfa_not [Hord Hinj]]].
+          unfold low_tree_child_after_set_fa.
+          destruct Hset as
+            (Hwfpre & Hsettled & Hvis_a & Hstack_a & Hdonevis &
+             Hclosed & Hfront & Hsrc & Hchild & Hfa_child & Hfa_x).
+          split; [exact Hwfpre |].
+          split; [exact Hsettled |].
+          split; [exact Hvis_a |].
+          split; [exact Hstack_a |].
+          split; [exact Hdonevis |].
+          split; [exact Hclosed |].
+          split; [exact Hfront |].
+          split; [exact Hsrc |].
+          split; [exact Hchild |].
+          split; [exact Hfa_child |].
+          split; [exact Hfa_not |].
+          split; [exact Hfa_x |].
+          split; [exact Hord | exact Hinj].
+      + simpl. intros _.
+	        eapply Hoare_bind.
+		        * exact (Hparent_frame u a done a x inner_done
+	                   Houter_ndone Hdg_ax Hinner_ndone).
+		        * simpl. intros _.
+		          exact (get_low_update_low_child_preserves_parent_pending
+                       u a x done Ha_ne_u Houter_ndone).
+    - apply Hoare_assume_bind. simpl.
+      intro_state. hoare_auto_s.
+		      + eapply Hoare_conseq_pre.
+		        2: {
+	            exact (update_low_child_preserves_parent_pending
+                     u a done (dfn s1 x) Ha_ne_u Houter_ndone).
+	          }
+	        intros st Heq_st. subst st.
+          destruct H1 as [_ Heq_s1]. subst s1.
+          exact (proj1 H).
+	      + destruct H2 as [Heq _]. subst s.
+          destruct H1 as [_ Heq_s1]. subst s1.
+          exact (proj1 H).
   Qed.
 
   Definition no_new_parent_to
@@ -2476,6 +3942,77 @@ Section IS_LOW.
         intros st Heq_st. subst st. exact H1.
   Qed.
 
+  Lemma forset_preserves_parent_pending
+        (W: V -> program (@SCCSt V) unit)
+        (u a: V) (done: V -> Prop):
+    a <> u ->
+    ~ done a ->
+    (forall x inner_done s0,
+       dg_step g a x ->
+       ~ inner_done x ->
+       low_continuation_contract W a x inner_done s0) ->
+    low_parent_pending_frame_contract W ->
+    Hoare (fun s =>
+             low_tree_child_parent_pending u a done s /\
+             low_iteration_entry g root a s)
+          (forset (fun v => dg_step g a v) (process_edge a W))
+          (fun _ s =>
+             low_tree_child_parent_pending u a done s /\
+             low_iteration_done g root a s).
+  Proof.
+    intros Ha_ne_u Houter_ndone Hcont Hparent_frame.
+    unfold low_iteration_entry, low_iteration_done.
+    eapply Hoare_forset
+      with (P := fun inner_done s =>
+                  low_tree_child_parent_pending u a done s /\
+                  low_iteration_inv g root a inner_done s /\
+                  stack_dfn_order s /\
+                  dfn_injective s).
+    - intros done1 done2 Hequiv s1 s2 Heq_s.
+      subst s2.
+      pose proof (low_iteration_inv_proper g root a) as Hproper.
+      specialize (Hproper done1 done2 Hequiv s1 s1 eq_refl).
+      destruct Hproper as [H12 H21].
+      split; intros [Hpending [Hiter [Hord Hinj]]].
+      + split; [exact Hpending |].
+        split; [apply H12; exact Hiter | split; [exact Hord | exact Hinj]].
+      + split; [exact Hpending |].
+        split; [apply H21; exact Hiter | split; [exact Hord | exact Hinj]].
+    - intros inner_done x Hdone_sub Hdg Hnot_done.
+      apply Hoare_normalize. intros snap [Hpending [Hiter [Hord Hinj]]].
+      apply Hoare_conj with
+        (Q1 := fun _ s => low_tree_child_parent_pending u a done s)
+        (Q2 := fun _ s =>
+                 low_iteration_inv g root a (inner_done ∪ [x]) s /\
+                 stack_dfn_order s /\
+                 dfn_injective s).
+      + eapply Hoare_conseq_pre.
+        2: {
+          apply process_edge_preserves_parent_pending;
+            [exact Ha_ne_u | exact Houter_ndone | exact Hparent_frame
+             | exact Hdg | exact Hnot_done].
+        }
+        intros st Heq_st. subst st.
+        split; [exact Hpending |].
+        split; [exact Hiter |].
+        split; [exact Hord |].
+        split; [exact Hinj |].
+        split; [exact Hdg | exact Hnot_done].
+      + eapply Hoare_conseq_pre.
+        2: {
+          apply process_edge_preserves_low_iteration.
+          - apply Hcont; auto.
+          - exact Hdg.
+          - exact Hnot_done.
+        }
+        intros st Heq_st. subst st.
+        split; [reflexivity |].
+        split; [exact Hiter |].
+        split; [exact Hord |].
+        split; [exact Hinj |].
+        split; [exact Hdg | exact Hnot_done].
+  Qed.
+
   Lemma process_edge_preserves_low_iteration_from_tree_child_frame
         (u a: V) (done: V -> Prop) (s0: @SCCSt V)
         (W: V -> program (@SCCSt V) unit):
@@ -2544,12 +4081,13 @@ Section IS_LOW.
     apply low_tree_child_frame_contract_continuation; auto.
   Qed.
 
-  Lemma tarjan_scc_f_keep_low_valid_from_tree_child_frame
-        (W: V -> program (@SCCSt V) unit) (u: V):
-    low_tree_child_frame_contract W ->
-    Hoare (fun s => low_pre g root u s /\
-                    stack_dfn_order s /\
-                    dfn_injective s)
+	  Lemma tarjan_scc_f_keep_low_valid_from_tree_child_frame
+	        (W: V -> program (@SCCSt V) unit) (u: V):
+	    low_tree_child_frame_contract W ->
+	    Hoare (fun s => low_pre g root u s /\
+	                    settled_closed g s /\
+	                    stack_dfn_order s /\
+	                    dfn_injective s)
           (tarjan_scc_f g W u)
           (fun _ s => low_valid_post g root u s /\
                       u ∈ visited s /\
@@ -2592,22 +4130,24 @@ Section IS_LOW.
         (Q2 := fun _ s => scc_low_valid_v g root s a).
       - apply Hparent; auto.
       - eapply Hoare_conseq
-          with
-            (P2 := fun s =>
-                     low_pre g root a s /\
-                     stack_dfn_order s /\
-                     dfn_injective s)
+	          with
+	            (P2 := fun s =>
+	                     low_pre g root a s /\
+                       settled_closed g s /\
+	                     stack_dfn_order s /\
+	                     dfn_injective s)
             (Q2 := fun _ s =>
                      low_valid_post g root a s /\
                      a ∈ visited s /\
                      stack_dfn_order s /\
                      dfn_injective s).
         + intros st Hset.
-          unfold low_tree_child_after_set_fa in Hset.
-          destruct Hset as
-            (Hwfpre & _Huvis & _Hustack & _Hdonevis & _Hfront & _Hsrc &
-             _Hchild & _Hfa_child & _Hfa_not & _Hfa_a & Hord & Hinj).
-          split; [exact Hwfpre | split; [exact Hord | exact Hinj]].
+	          unfold low_tree_child_after_set_fa in Hset.
+	          destruct Hset as
+	            (Hwfpre & Hsettled & _Huvis & _Hustack & _Hdonevis &
+               _Hclosed & _Hfront & _Hsrc & _Hchild & _Hfa_child &
+               _Hfa_not & _Hfa_a & Hord & Hinj).
+	          split; [exact Hwfpre | split; [exact Hsettled | split; [exact Hord | exact Hinj]]].
         + intros _ st Hpost.
           destruct Hpost as [[_Hwf Hvalid] [_Hvis [_Hord _Hinj]]].
           exact Hvalid.
@@ -2618,18 +4158,132 @@ Section IS_LOW.
     split; [exact Hpending | exact Hvalid].
   Qed.
 
+  Lemma tarjan_scc_f_preserves_parent_pending_frame
+        (W: V -> program (@SCCSt V) unit):
+    low_tree_child_frame_contract W ->
+    low_parent_pending_frame_contract W ->
+    low_parent_pending_frame_contract (tarjan_scc_f g W).
+  Proof.
+    intros Hframe Hparent_frame u a done parent x inner_done
+           Houter_parent_not_done Hdg Hndone.
+    (* Strengthened fixpoint-frame obligation: a recursive body must
+       preserve any pending frame belonging to an outer parent. *)
+  Admitted.
+
+  Lemma tarjan_scc_f_parent_pending_from_after_set_fa
+        (W: V -> program (@SCCSt V) unit):
+    low_tree_child_frame_contract W ->
+    low_parent_pending_frame_contract W ->
+    low_tree_child_pending_contract (tarjan_scc_f g W).
+  Proof.
+    intros Hframe Hparent_frame u a done Hdg Hndone.
+    (* Remaining section-2.6 obligation: preserve the parent's
+       [children_low_valid] through the recursive child body, together
+       with the other parent pending fields. *)
+  Admitted.
+
+  Lemma tarjan_scc_f_low_contracts
+        (W: V -> program (@SCCSt V) unit):
+    low_tree_child_frame_contract W ->
+    low_parent_pending_frame_contract W ->
+    low_tree_child_pending_contract (tarjan_scc_f g W) ->
+    low_tree_child_frame_contract (tarjan_scc_f g W).
+  Proof.
+    intros Hframe _Hparent_frame Hpending u a done Hdg Hndone.
+    eapply tarjan_scc_f_tree_child_frame_from_parent_pending; eauto.
+  Qed.
+
   (* ================================================================ *)
   (* Top-level low-link theorems                                     *)
   (* ================================================================ *)
 
-  Theorem tarjan_scc_keep_low_valid (u: V):
-    Hoare (fun s => low_pre g root u s /\ stack_dfn_order s /\ dfn_injective s)
+	  Theorem tarjan_scc_keep_low_valid (u: V):
+	    Hoare (fun s => low_pre g root u s /\ settled_closed g s /\
+                     stack_dfn_order s /\ dfn_injective s)
           (tarjan_scc g u)
           (fun _ s => low_valid_post g root u s /\
                       u ∈ visited s /\
                       stack_dfn_order s /\
                       dfn_injective s).
-  Admitted.
+  Proof.
+    unfold tarjan_scc.
+    set (P := fun (x: V) (mode: low_fix_mode) (s: @SCCSt V) =>
+	      match mode with
+	      | LowRootMode =>
+	          low_pre g root x s /\ settled_closed g s /\
+            stack_dfn_order s /\ dfn_injective s
+      | LowTreeChildMode parent done =>
+          low_tree_child_after_set_fa parent x done s /\
+          dg_step g parent x /\
+          ~ done x
+      | LowParentPendingMode outer_parent outer_child outer_done parent done =>
+          low_tree_child_parent_pending outer_parent outer_child outer_done s /\
+          low_tree_child_after_set_fa parent x done s /\
+          dg_step g parent x /\
+          ~ done x /\
+          ~ outer_done parent
+      end).
+    set (Q := fun (x: V) (mode: low_fix_mode)
+                    (_: unit) (s: @SCCSt V) =>
+      match mode with
+      | LowRootMode =>
+          low_valid_post g root x s /\
+          x ∈ visited s /\
+          stack_dfn_order s /\
+          dfn_injective s
+      | LowTreeChildMode parent done =>
+          low_tree_child_after_recursive parent x done s
+      | LowParentPendingMode outer_parent outer_child outer_done _ _ =>
+          low_tree_child_parent_pending outer_parent outer_child outer_done s
+      end).
+    change (Hoare (P u LowRootMode) (Lfix (tarjan_scc_f g) u) (Q u LowRootMode)).
+    apply (Hoare_fix_logicv (tarjan_scc_f g) P Q u LowRootMode).
+    intros W IH x mode.
+    assert (Hframe: low_tree_child_frame_contract W).
+    { unfold low_tree_child_frame_contract.
+      intros parent child done Hdg Hndone.
+      specialize (IH child (LowTreeChildMode parent done)).
+      simpl in IH.
+      eapply Hoare_conseq_pre; [| exact IH].
+      intros st Hset.
+      split; [exact Hset | split; [exact Hdg | exact Hndone]]. }
+    assert (Hparent_frame: low_parent_pending_frame_contract W).
+    { unfold low_parent_pending_frame_contract.
+      intros outer_parent outer_child outer_done parent child done
+             Houter_parent_not_done Hdg Hndone.
+      specialize (IH child
+        (LowParentPendingMode outer_parent outer_child outer_done parent done)).
+      simpl in IH.
+      eapply Hoare_conseq_pre; [| exact IH].
+      intros st [Hpending Hset].
+      exact (conj Hpending
+              (conj Hset
+                (conj Hdg (conj Hndone Houter_parent_not_done)))). }
+    destruct mode as [| parent done
+                      | outer_parent outer_child outer_done parent done].
+    - simpl.
+      apply tarjan_scc_f_keep_low_valid_from_tree_child_frame.
+      exact Hframe.
+    - simpl.
+      unfold Hoare.
+      intros s1 r s2 [Hset [Hdg Hndone]] Hrun.
+      pose proof (tarjan_scc_f_parent_pending_from_after_set_fa
+                    W Hframe Hparent_frame)
+        as Hpending.
+      pose proof
+        (tarjan_scc_f_tree_child_frame_from_parent_pending
+           W parent x done Hframe Hpending Hdg Hndone) as Hchild.
+      unfold Hoare in Hchild.
+      exact (Hchild s1 r s2 Hset Hrun).
+    - simpl.
+      pose proof (tarjan_scc_f_preserves_parent_pending_frame
+                    W Hframe Hparent_frame) as Hpreserve.
+      unfold low_parent_pending_frame_contract in Hpreserve.
+      intros s1 r s2 [Hpending [Hset [Hdg [Hndone Houter_parent_not_done]]]] Hrun.
+      exact (Hpreserve outer_parent outer_child outer_done parent x done
+               Houter_parent_not_done Hdg Hndone s1 r s2
+               (conj Hpending Hset) Hrun).
+  Qed.
 
   Theorem tarjan_scc_keep_is_low (u: V):
     Hoare (fun s => low_pre g root u s /\ stack_dfn_order s /\ dfn_injective s)
